QCP_examples/humaneval/spec_logic_rewrite_c_files/C_6_goal.v
@@ -1,0 +1,1313 @@
+Require Import Coq.ZArith.ZArith.
+Require Import Coq.Bool.Bool.
+Require Import Coq.Strings.String.
+Require Import Coq.Strings.Ascii.
+Require Import Coq.Lists.List.
+Require Import Coq.Classes.RelationClasses.
+Require Import Coq.Classes.Morphisms.
+Require Import Coq.micromega.Psatz.
+Require Import Coq.Sorting.Permutation.
+From AUXLib Require Import int_auto Axioms Feq Idents ListLib VMap.
+Require Import SetsClass.SetsClass. Import SetsNotation.
+From SimpleC.SL Require Import Mem SeparationLogic.
+Require Import Logic.LogicGenerator.demo932.Interface.
+Local Open Scope Z_scope.
+Local Open Scope sets.
+Local Open Scope string_scope.
+Local Open Scope list.
+Import naive_C_Rules.
+Require Import SimpleC.StdLib.string_lib.
+Require Import coins_6.
+Local Open Scope sac.
+From SimpleC.EE.QCP_demos_LLM Require Import int_array_strategy_goal.
+From SimpleC.EE.QCP_demos_LLM Require Import int_array_strategy_proof.
+From SimpleC.EE.QCP_demos_LLM Require Import uint_array_strategy_goal.
+From SimpleC.EE.QCP_demos_LLM Require Import uint_array_strategy_proof.
+From SimpleC.EE.QCP_demos_LLM Require Import undef_uint_array_strategy_goal.
+From SimpleC.EE.QCP_demos_LLM Require Import undef_uint_array_strategy_proof.
+From SimpleC.EE.QCP_demos_LLM Require Import array_shape_strategy_goal.
+From SimpleC.EE.QCP_demos_LLM Require Import array_shape_strategy_proof.
+From SimpleC.EE.QCP_demos_LLM Require Import char_array_strategy_goal.
+From SimpleC.EE.QCP_demos_LLM Require Import char_array_strategy_proof.
+From SimpleC.StdLib Require Import string_strategy_goal.
+From SimpleC.StdLib Require Import string_strategy_proof.
+
+(*----- Function parse_nested_parens -----*)
+
+Definition parse_nested_parens_safety_wit_1 := 
+forall (paren_string_pre: Z) (str_l: (@list Z)) (retval: Z) (retval_2: Z) (PreH1 : (retval_2 <> 0)) (PreH2 : (retval = (string_length (str_l)))) (PreH3 : (0 <= ((string_length (str_l)) + 1 ))) (PreH4 : (valid_string str_l )) (PreH5 : (all_ascii str_l )) (PreH6 : (valid_paren_depth_input_6 str_l )) (PreH7 : (parse_safe_input_6 str_l )) (PreH8 : (((string_length (str_l)) + 1 ) < INT_MAX)) (PreH9 : (problem_6_pre_z str_l )) ,
+  ((( &( "cap" ) )) # Int  |->_)
+  **  ((&((retval_2)  # "<anonymous struct>" ->ₛ "data")) # Ptr  |->_)
+  **  ((&((retval_2)  # "<anonymous struct>" ->ₛ "size")) # Int  |->_)
+  **  (CharArray.full paren_string_pre ((string_length (str_l)) + 1 ) (c_string (str_l)) )
+  **  ((( &( "out" ) )) # Ptr  |-> retval_2)
+  **  ((( &( "n" ) )) # Int  |-> retval)
+  **  ((( &( "paren_string" ) )) # Ptr  |-> paren_string_pre)
+|--
+  “ ((retval + 1 ) <= INT_MAX) ” 
+  &&  “ ((INT_MIN) <= (retval + 1 )) ”
+.
+
+Definition parse_nested_parens_safety_wit_2 := 
+forall (paren_string_pre: Z) (str_l: (@list Z)) (retval: Z) (retval_2: Z) (PreH1 : (retval_2 <> 0)) (PreH2 : (retval = (string_length (str_l)))) (PreH3 : (0 <= ((string_length (str_l)) + 1 ))) (PreH4 : (valid_string str_l )) (PreH5 : (all_ascii str_l )) (PreH6 : (valid_paren_depth_input_6 str_l )) (PreH7 : (parse_safe_input_6 str_l )) (PreH8 : (((string_length (str_l)) + 1 ) < INT_MAX)) (PreH9 : (problem_6_pre_z str_l )) ,
+  ((( &( "cap" ) )) # Int  |->_)
+  **  ((&((retval_2)  # "<anonymous struct>" ->ₛ "data")) # Ptr  |->_)
+  **  ((&((retval_2)  # "<anonymous struct>" ->ₛ "size")) # Int  |->_)
+  **  (CharArray.full paren_string_pre ((string_length (str_l)) + 1 ) (c_string (str_l)) )
+  **  ((( &( "out" ) )) # Ptr  |-> retval_2)
+  **  ((( &( "n" ) )) # Int  |-> retval)
+  **  ((( &( "paren_string" ) )) # Ptr  |-> paren_string_pre)
+|--
+  “ (1 <= INT_MAX) ” 
+  &&  “ ((INT_MIN) <= 1) ”
+.
+
+Definition parse_nested_parens_safety_wit_3 := 
+forall (paren_string_pre: Z) (str_l: (@list Z)) (retval: Z) (retval_2: Z) (retval_3: Z) (PreH1 : (retval_3 <> 0)) (PreH2 : (retval_2 <> 0)) (PreH3 : (retval = (string_length (str_l)))) (PreH4 : (0 <= ((string_length (str_l)) + 1 ))) (PreH5 : (valid_string str_l )) (PreH6 : (all_ascii str_l )) (PreH7 : (valid_paren_depth_input_6 str_l )) (PreH8 : (parse_safe_input_6 str_l )) (PreH9 : (((string_length (str_l)) + 1 ) < INT_MAX)) (PreH10 : (problem_6_pre_z str_l )) ,
+  ((( &( "level" ) )) # Int  |->_)
+  **  (IntArray.undef_full retval_3 (retval + 1 ) )
+  **  ((( &( "data" ) )) # Ptr  |-> retval_3)
+  **  ((( &( "cap" ) )) # Int  |-> (retval + 1 ))
+  **  ((&((retval_2)  # "<anonymous struct>" ->ₛ "data")) # Ptr  |->_)
+  **  ((&((retval_2)  # "<anonymous struct>" ->ₛ "size")) # Int  |->_)
+  **  (CharArray.full paren_string_pre ((string_length (str_l)) + 1 ) (c_string (str_l)) )
+  **  ((( &( "out" ) )) # Ptr  |-> retval_2)
+  **  ((( &( "n" ) )) # Int  |-> retval)
+  **  ((( &( "paren_string" ) )) # Ptr  |-> paren_string_pre)
+|--
+  “ (0 <= INT_MAX) ” 
+  &&  “ ((INT_MIN) <= 0) ”
+.
+
+Definition parse_nested_parens_safety_wit_4 := 
+forall (paren_string_pre: Z) (str_l: (@list Z)) (retval: Z) (retval_2: Z) (retval_3: Z) (PreH1 : (retval_3 <> 0)) (PreH2 : (retval_2 <> 0)) (PreH3 : (retval = (string_length (str_l)))) (PreH4 : (0 <= ((string_length (str_l)) + 1 ))) (PreH5 : (valid_string str_l )) (PreH6 : (all_ascii str_l )) (PreH7 : (valid_paren_depth_input_6 str_l )) (PreH8 : (parse_safe_input_6 str_l )) (PreH9 : (((string_length (str_l)) + 1 ) < INT_MAX)) (PreH10 : (problem_6_pre_z str_l )) ,
+  ((( &( "max_level" ) )) # Int  |->_)
+  **  ((( &( "level" ) )) # Int  |-> 0)
+  **  (IntArray.undef_full retval_3 (retval + 1 ) )
+  **  ((( &( "data" ) )) # Ptr  |-> retval_3)
+  **  ((( &( "cap" ) )) # Int  |-> (retval + 1 ))
+  **  ((&((retval_2)  # "<anonymous struct>" ->ₛ "data")) # Ptr  |->_)
+  **  ((&((retval_2)  # "<anonymous struct>" ->ₛ "size")) # Int  |->_)
+  **  (CharArray.full paren_string_pre ((string_length (str_l)) + 1 ) (c_string (str_l)) )
+  **  ((( &( "out" ) )) # Ptr  |-> retval_2)
+  **  ((( &( "n" ) )) # Int  |-> retval)
+  **  ((( &( "paren_string" ) )) # Ptr  |-> paren_string_pre)
+|--
+  “ (0 <= INT_MAX) ” 
+  &&  “ ((INT_MIN) <= 0) ”
+.
+
+Definition parse_nested_parens_safety_wit_5 := 
+forall (paren_string_pre: Z) (str_l: (@list Z)) (retval: Z) (retval_2: Z) (retval_3: Z) (PreH1 : (retval_3 <> 0)) (PreH2 : (retval_2 <> 0)) (PreH3 : (retval = (string_length (str_l)))) (PreH4 : (0 <= ((string_length (str_l)) + 1 ))) (PreH5 : (valid_string str_l )) (PreH6 : (all_ascii str_l )) (PreH7 : (valid_paren_depth_input_6 str_l )) (PreH8 : (parse_safe_input_6 str_l )) (PreH9 : (((string_length (str_l)) + 1 ) < INT_MAX)) (PreH10 : (problem_6_pre_z str_l )) ,
+  ((( &( "out_size" ) )) # Int  |->_)
+  **  ((( &( "max_level" ) )) # Int  |-> 0)
+  **  ((( &( "level" ) )) # Int  |-> 0)
+  **  (IntArray.undef_full retval_3 (retval + 1 ) )
+  **  ((( &( "data" ) )) # Ptr  |-> retval_3)
+  **  ((( &( "cap" ) )) # Int  |-> (retval + 1 ))
+  **  ((&((retval_2)  # "<anonymous struct>" ->ₛ "data")) # Ptr  |->_)
+  **  ((&((retval_2)  # "<anonymous struct>" ->ₛ "size")) # Int  |->_)
+  **  (CharArray.full paren_string_pre ((string_length (str_l)) + 1 ) (c_string (str_l)) )
+  **  ((( &( "out" ) )) # Ptr  |-> retval_2)
+  **  ((( &( "n" ) )) # Int  |-> retval)
+  **  ((( &( "paren_string" ) )) # Ptr  |-> paren_string_pre)
+|--
+  “ (0 <= INT_MAX) ” 
+  &&  “ ((INT_MIN) <= 0) ”
+.
+
+Definition parse_nested_parens_safety_wit_6 := 
+forall (paren_string_pre: Z) (str_l: (@list Z)) (retval: Z) (retval_2: Z) (retval_3: Z) (PreH1 : (retval_3 <> 0)) (PreH2 : (retval_2 <> 0)) (PreH3 : (retval = (string_length (str_l)))) (PreH4 : (0 <= ((string_length (str_l)) + 1 ))) (PreH5 : (valid_string str_l )) (PreH6 : (all_ascii str_l )) (PreH7 : (valid_paren_depth_input_6 str_l )) (PreH8 : (parse_safe_input_6 str_l )) (PreH9 : (((string_length (str_l)) + 1 ) < INT_MAX)) (PreH10 : (problem_6_pre_z str_l )) ,
+  ((( &( "ch" ) )) # Int  |->_)
+  **  ((( &( "out_size" ) )) # Int  |-> 0)
+  **  ((( &( "max_level" ) )) # Int  |-> 0)
+  **  ((( &( "level" ) )) # Int  |-> 0)
+  **  (IntArray.undef_full retval_3 (retval + 1 ) )
+  **  ((( &( "data" ) )) # Ptr  |-> retval_3)
+  **  ((( &( "cap" ) )) # Int  |-> (retval + 1 ))
+  **  ((&((retval_2)  # "<anonymous struct>" ->ₛ "data")) # Ptr  |->_)
+  **  ((&((retval_2)  # "<anonymous struct>" ->ₛ "size")) # Int  |->_)
+  **  (CharArray.full paren_string_pre ((string_length (str_l)) + 1 ) (c_string (str_l)) )
+  **  ((( &( "out" ) )) # Ptr  |-> retval_2)
+  **  ((( &( "n" ) )) # Int  |-> retval)
+  **  ((( &( "paren_string" ) )) # Ptr  |-> paren_string_pre)
+|--
+  “ (0 <= INT_MAX) ” 
+  &&  “ ((INT_MIN) <= 0) ”
+.
+
+Definition parse_nested_parens_safety_wit_7 := 
+forall (paren_string_pre: Z) (str_l: (@list Z)) (retval: Z) (retval_2: Z) (retval_3: Z) (PreH1 : (retval_3 <> 0)) (PreH2 : (retval_2 <> 0)) (PreH3 : (retval = (string_length (str_l)))) (PreH4 : (0 <= ((string_length (str_l)) + 1 ))) (PreH5 : (valid_string str_l )) (PreH6 : (all_ascii str_l )) (PreH7 : (valid_paren_depth_input_6 str_l )) (PreH8 : (parse_safe_input_6 str_l )) (PreH9 : (((string_length (str_l)) + 1 ) < INT_MAX)) (PreH10 : (problem_6_pre_z str_l )) ,
+  ((( &( "i" ) )) # Int  |->_)
+  **  ((( &( "ch" ) )) # Int  |-> 0)
+  **  ((( &( "out_size" ) )) # Int  |-> 0)
+  **  ((( &( "max_level" ) )) # Int  |-> 0)
+  **  ((( &( "level" ) )) # Int  |-> 0)
+  **  (IntArray.undef_full retval_3 (retval + 1 ) )
+  **  ((( &( "data" ) )) # Ptr  |-> retval_3)
+  **  ((( &( "cap" ) )) # Int  |-> (retval + 1 ))
+  **  ((&((retval_2)  # "<anonymous struct>" ->ₛ "data")) # Ptr  |->_)
+  **  ((&((retval_2)  # "<anonymous struct>" ->ₛ "size")) # Int  |->_)
+  **  (CharArray.full paren_string_pre ((string_length (str_l)) + 1 ) (c_string (str_l)) )
+  **  ((( &( "out" ) )) # Ptr  |-> retval_2)
+  **  ((( &( "n" ) )) # Int  |-> retval)
+  **  ((( &( "paren_string" ) )) # Ptr  |-> paren_string_pre)
+|--
+  “ (0 <= INT_MAX) ” 
+  &&  “ ((INT_MIN) <= 0) ”
+.
+
+Definition parse_nested_parens_safety_wit_8 := 
+forall (paren_string_pre: Z) (str_l: (@list Z)) (ch: Z) (max_level: Z) (level: Z) (output_l: (@list Z)) (out_size: Z) (data: Z) (out: Z) (cap: Z) (n: Z) (i: Z) (PreH1 : (i < n)) (PreH2 : (0 <= i)) (PreH3 : (i <= n)) (PreH4 : (n = (string_length (str_l)))) (PreH5 : (cap = (n + 1 ))) (PreH6 : (out <> 0)) (PreH7 : (data <> 0)) (PreH8 : (0 <= out_size)) (PreH9 : (out_size <= i)) (PreH10 : (out_size = (Zlength (output_l)))) (PreH11 : (0 <= level)) (PreH12 : (level <= i)) (PreH13 : (0 <= max_level)) (PreH14 : (max_level <= i)) (PreH15 : (0 <= ch)) (PreH16 : (ch <= 127)) (PreH17 : (valid_string str_l )) (PreH18 : (all_ascii str_l )) (PreH19 : (valid_paren_depth_input_6 str_l )) (PreH20 : (parse_safe_input_6 str_l )) (PreH21 : (((string_length (str_l)) + 1 ) < INT_MAX)) (PreH22 : (problem_6_pre_z str_l )) (PreH23 : (parse_state_6 str_l i level max_level output_l )) ,
+  ((( &( "i" ) )) # Int  |-> i)
+  **  ((( &( "n" ) )) # Int  |-> n)
+  **  ((( &( "cap" ) )) # Int  |-> cap)
+  **  ((( &( "paren_string" ) )) # Ptr  |-> paren_string_pre)
+  **  ((( &( "out" ) )) # Ptr  |-> out)
+  **  ((( &( "data" ) )) # Ptr  |-> data)
+  **  ((( &( "out_size" ) )) # Int  |-> out_size)
+  **  ((( &( "level" ) )) # Int  |-> level)
+  **  ((( &( "max_level" ) )) # Int  |-> max_level)
+  **  ((( &( "ch" ) )) # Int  |-> (Znth i (c_string (str_l)) 0))
+  **  (store_string paren_string_pre str_l )
+  **  ((&((out)  # "<anonymous struct>" ->ₛ "data")) # Ptr  |->_)
+  **  ((&((out)  # "<anonymous struct>" ->ₛ "size")) # Int  |->_)
+  **  (IntArray.seg data 0 out_size output_l )
+  **  (IntArray.undef_seg data out_size cap )
+|--
+  “ (40 <= INT_MAX) ” 
+  &&  “ ((INT_MIN) <= 40) ”
+.
+
+Definition parse_nested_parens_safety_wit_9 := 
+forall (paren_string_pre: Z) (str_l: (@list Z)) (ch: Z) (max_level: Z) (level: Z) (output_l: (@list Z)) (out_size: Z) (data: Z) (out: Z) (cap: Z) (n: Z) (i: Z) (PreH1 : ((Znth i (c_string (str_l)) 0) = 40)) (PreH2 : (i < n)) (PreH3 : (0 <= i)) (PreH4 : (i <= n)) (PreH5 : (n = (string_length (str_l)))) (PreH6 : (cap = (n + 1 ))) (PreH7 : (out <> 0)) (PreH8 : (data <> 0)) (PreH9 : (0 <= out_size)) (PreH10 : (out_size <= i)) (PreH11 : (out_size = (Zlength (output_l)))) (PreH12 : (0 <= level)) (PreH13 : (level <= i)) (PreH14 : (0 <= max_level)) (PreH15 : (max_level <= i)) (PreH16 : (0 <= ch)) (PreH17 : (ch <= 127)) (PreH18 : (valid_string str_l )) (PreH19 : (all_ascii str_l )) (PreH20 : (valid_paren_depth_input_6 str_l )) (PreH21 : (parse_safe_input_6 str_l )) (PreH22 : (((string_length (str_l)) + 1 ) < INT_MAX)) (PreH23 : (problem_6_pre_z str_l )) (PreH24 : (parse_state_6 str_l i level max_level output_l )) ,
+  ((( &( "i" ) )) # Int  |-> i)
+  **  ((( &( "n" ) )) # Int  |-> n)
+  **  ((( &( "cap" ) )) # Int  |-> cap)
+  **  ((( &( "paren_string" ) )) # Ptr  |-> paren_string_pre)
+  **  ((( &( "out" ) )) # Ptr  |-> out)
+  **  ((( &( "data" ) )) # Ptr  |-> data)
+  **  ((( &( "out_size" ) )) # Int  |-> out_size)
+  **  ((( &( "level" ) )) # Int  |-> level)
+  **  ((( &( "max_level" ) )) # Int  |-> max_level)
+  **  ((( &( "ch" ) )) # Int  |-> (Znth i (c_string (str_l)) 0))
+  **  (store_string paren_string_pre str_l )
+  **  ((&((out)  # "<anonymous struct>" ->ₛ "data")) # Ptr  |->_)
+  **  ((&((out)  # "<anonymous struct>" ->ₛ "size")) # Int  |->_)
+  **  (IntArray.seg data 0 out_size output_l )
+  **  (IntArray.undef_seg data out_size cap )
+|--
+  “ ((level + 1 ) <= INT_MAX) ” 
+  &&  “ ((INT_MIN) <= (level + 1 )) ”
+.
+
+Definition parse_nested_parens_safety_wit_10 := 
+forall (paren_string_pre: Z) (str_l: (@list Z)) (ch: Z) (max_level: Z) (level: Z) (output_l: (@list Z)) (out_size: Z) (data: Z) (out: Z) (cap: Z) (n: Z) (i: Z) (PreH1 : ((Znth i (c_string (str_l)) 0) = 40)) (PreH2 : (i < n)) (PreH3 : (0 <= i)) (PreH4 : (i <= n)) (PreH5 : (n = (string_length (str_l)))) (PreH6 : (cap = (n + 1 ))) (PreH7 : (out <> 0)) (PreH8 : (data <> 0)) (PreH9 : (0 <= out_size)) (PreH10 : (out_size <= i)) (PreH11 : (out_size = (Zlength (output_l)))) (PreH12 : (0 <= level)) (PreH13 : (level <= i)) (PreH14 : (0 <= max_level)) (PreH15 : (max_level <= i)) (PreH16 : (0 <= ch)) (PreH17 : (ch <= 127)) (PreH18 : (valid_string str_l )) (PreH19 : (all_ascii str_l )) (PreH20 : (valid_paren_depth_input_6 str_l )) (PreH21 : (parse_safe_input_6 str_l )) (PreH22 : (((string_length (str_l)) + 1 ) < INT_MAX)) (PreH23 : (problem_6_pre_z str_l )) (PreH24 : (parse_state_6 str_l i level max_level output_l )) ,
+  ((( &( "i" ) )) # Int  |-> i)
+  **  ((( &( "n" ) )) # Int  |-> n)
+  **  ((( &( "cap" ) )) # Int  |-> cap)
+  **  ((( &( "paren_string" ) )) # Ptr  |-> paren_string_pre)
+  **  ((( &( "out" ) )) # Ptr  |-> out)
+  **  ((( &( "data" ) )) # Ptr  |-> data)
+  **  ((( &( "out_size" ) )) # Int  |-> out_size)
+  **  ((( &( "level" ) )) # Int  |-> level)
+  **  ((( &( "max_level" ) )) # Int  |-> max_level)
+  **  ((( &( "ch" ) )) # Int  |-> (Znth i (c_string (str_l)) 0))
+  **  (store_string paren_string_pre str_l )
+  **  ((&((out)  # "<anonymous struct>" ->ₛ "data")) # Ptr  |->_)
+  **  ((&((out)  # "<anonymous struct>" ->ₛ "size")) # Int  |->_)
+  **  (IntArray.seg data 0 out_size output_l )
+  **  (IntArray.undef_seg data out_size cap )
+|--
+  “ (1 <= INT_MAX) ” 
+  &&  “ ((INT_MIN) <= 1) ”
+.
+
+Definition parse_nested_parens_safety_wit_11 := 
+forall (paren_string_pre: Z) (str_l: (@list Z)) (ch: Z) (max_level: Z) (level: Z) (output_l: (@list Z)) (out_size: Z) (data: Z) (out: Z) (cap: Z) (n: Z) (i: Z) (PreH1 : ((Znth i (c_string (str_l)) 0) <> 40)) (PreH2 : (i < n)) (PreH3 : (0 <= i)) (PreH4 : (i <= n)) (PreH5 : (n = (string_length (str_l)))) (PreH6 : (cap = (n + 1 ))) (PreH7 : (out <> 0)) (PreH8 : (data <> 0)) (PreH9 : (0 <= out_size)) (PreH10 : (out_size <= i)) (PreH11 : (out_size = (Zlength (output_l)))) (PreH12 : (0 <= level)) (PreH13 : (level <= i)) (PreH14 : (0 <= max_level)) (PreH15 : (max_level <= i)) (PreH16 : (0 <= ch)) (PreH17 : (ch <= 127)) (PreH18 : (valid_string str_l )) (PreH19 : (all_ascii str_l )) (PreH20 : (valid_paren_depth_input_6 str_l )) (PreH21 : (parse_safe_input_6 str_l )) (PreH22 : (((string_length (str_l)) + 1 ) < INT_MAX)) (PreH23 : (problem_6_pre_z str_l )) (PreH24 : (parse_state_6 str_l i level max_level output_l )) ,
+  ((( &( "i" ) )) # Int  |-> i)
+  **  ((( &( "n" ) )) # Int  |-> n)
+  **  ((( &( "cap" ) )) # Int  |-> cap)
+  **  ((( &( "paren_string" ) )) # Ptr  |-> paren_string_pre)
+  **  ((( &( "out" ) )) # Ptr  |-> out)
+  **  ((( &( "data" ) )) # Ptr  |-> data)
+  **  ((( &( "out_size" ) )) # Int  |-> out_size)
+  **  ((( &( "level" ) )) # Int  |-> level)
+  **  ((( &( "max_level" ) )) # Int  |-> max_level)
+  **  ((( &( "ch" ) )) # Int  |-> (Znth i (c_string (str_l)) 0))
+  **  (store_string paren_string_pre str_l )
+  **  ((&((out)  # "<anonymous struct>" ->ₛ "data")) # Ptr  |->_)
+  **  ((&((out)  # "<anonymous struct>" ->ₛ "size")) # Int  |->_)
+  **  (IntArray.seg data 0 out_size output_l )
+  **  (IntArray.undef_seg data out_size cap )
+|--
+  “ (41 <= INT_MAX) ” 
+  &&  “ ((INT_MIN) <= 41) ”
+.
+
+Definition parse_nested_parens_safety_wit_12 := 
+forall (paren_string_pre: Z) (str_l: (@list Z)) (ch: Z) (max_level: Z) (level: Z) (output_l: (@list Z)) (out_size: Z) (data: Z) (out: Z) (cap: Z) (n: Z) (i: Z) (PreH1 : ((Znth i (c_string (str_l)) 0) = 41)) (PreH2 : ((Znth i (c_string (str_l)) 0) <> 40)) (PreH3 : (i < n)) (PreH4 : (0 <= i)) (PreH5 : (i <= n)) (PreH6 : (n = (string_length (str_l)))) (PreH7 : (cap = (n + 1 ))) (PreH8 : (out <> 0)) (PreH9 : (data <> 0)) (PreH10 : (0 <= out_size)) (PreH11 : (out_size <= i)) (PreH12 : (out_size = (Zlength (output_l)))) (PreH13 : (0 <= level)) (PreH14 : (level <= i)) (PreH15 : (0 <= max_level)) (PreH16 : (max_level <= i)) (PreH17 : (0 <= ch)) (PreH18 : (ch <= 127)) (PreH19 : (valid_string str_l )) (PreH20 : (all_ascii str_l )) (PreH21 : (valid_paren_depth_input_6 str_l )) (PreH22 : (parse_safe_input_6 str_l )) (PreH23 : (((string_length (str_l)) + 1 ) < INT_MAX)) (PreH24 : (problem_6_pre_z str_l )) (PreH25 : (parse_state_6 str_l i level max_level output_l )) ,
+  ((( &( "i" ) )) # Int  |-> i)
+  **  ((( &( "n" ) )) # Int  |-> n)
+  **  ((( &( "cap" ) )) # Int  |-> cap)
+  **  ((( &( "paren_string" ) )) # Ptr  |-> paren_string_pre)
+  **  ((( &( "out" ) )) # Ptr  |-> out)
+  **  ((( &( "data" ) )) # Ptr  |-> data)
+  **  ((( &( "out_size" ) )) # Int  |-> out_size)
+  **  ((( &( "level" ) )) # Int  |-> level)
+  **  ((( &( "max_level" ) )) # Int  |-> max_level)
+  **  ((( &( "ch" ) )) # Int  |-> (Znth i (c_string (str_l)) 0))
+  **  (store_string paren_string_pre str_l )
+  **  ((&((out)  # "<anonymous struct>" ->ₛ "data")) # Ptr  |->_)
+  **  ((&((out)  # "<anonymous struct>" ->ₛ "size")) # Int  |->_)
+  **  (IntArray.seg data 0 out_size output_l )
+  **  (IntArray.undef_seg data out_size cap )
+|--
+  “ ((level - 1 ) <= INT_MAX) ” 
+  &&  “ ((INT_MIN) <= (level - 1 )) ”
+.
+
+Definition parse_nested_parens_safety_wit_13 := 
+forall (paren_string_pre: Z) (str_l: (@list Z)) (ch: Z) (max_level: Z) (level: Z) (output_l: (@list Z)) (out_size: Z) (data: Z) (out: Z) (cap: Z) (n: Z) (i: Z) (PreH1 : ((Znth i (c_string (str_l)) 0) = 41)) (PreH2 : ((Znth i (c_string (str_l)) 0) <> 40)) (PreH3 : (i < n)) (PreH4 : (0 <= i)) (PreH5 : (i <= n)) (PreH6 : (n = (string_length (str_l)))) (PreH7 : (cap = (n + 1 ))) (PreH8 : (out <> 0)) (PreH9 : (data <> 0)) (PreH10 : (0 <= out_size)) (PreH11 : (out_size <= i)) (PreH12 : (out_size = (Zlength (output_l)))) (PreH13 : (0 <= level)) (PreH14 : (level <= i)) (PreH15 : (0 <= max_level)) (PreH16 : (max_level <= i)) (PreH17 : (0 <= ch)) (PreH18 : (ch <= 127)) (PreH19 : (valid_string str_l )) (PreH20 : (all_ascii str_l )) (PreH21 : (valid_paren_depth_input_6 str_l )) (PreH22 : (parse_safe_input_6 str_l )) (PreH23 : (((string_length (str_l)) + 1 ) < INT_MAX)) (PreH24 : (problem_6_pre_z str_l )) (PreH25 : (parse_state_6 str_l i level max_level output_l )) ,
+  ((( &( "i" ) )) # Int  |-> i)
+  **  ((( &( "n" ) )) # Int  |-> n)
+  **  ((( &( "cap" ) )) # Int  |-> cap)
+  **  ((( &( "paren_string" ) )) # Ptr  |-> paren_string_pre)
+  **  ((( &( "out" ) )) # Ptr  |-> out)
+  **  ((( &( "data" ) )) # Ptr  |-> data)
+  **  ((( &( "out_size" ) )) # Int  |-> out_size)
+  **  ((( &( "level" ) )) # Int  |-> level)
+  **  ((( &( "max_level" ) )) # Int  |-> max_level)
+  **  ((( &( "ch" ) )) # Int  |-> (Znth i (c_string (str_l)) 0))
+  **  (store_string paren_string_pre str_l )
+  **  ((&((out)  # "<anonymous struct>" ->ₛ "data")) # Ptr  |->_)
+  **  ((&((out)  # "<anonymous struct>" ->ₛ "size")) # Int  |->_)
+  **  (IntArray.seg data 0 out_size output_l )
+  **  (IntArray.undef_seg data out_size cap )
+|--
+  “ (1 <= INT_MAX) ” 
+  &&  “ ((INT_MIN) <= 1) ”
+.
+
+Definition parse_nested_parens_safety_wit_14 := 
+forall (paren_string_pre: Z) (str_l: (@list Z)) (ch: Z) (max_level: Z) (level: Z) (output_l: (@list Z)) (out_size: Z) (data: Z) (out: Z) (cap: Z) (n: Z) (i: Z) (PreH1 : ((Znth i (c_string (str_l)) 0) = 41)) (PreH2 : ((Znth i (c_string (str_l)) 0) <> 40)) (PreH3 : (i < n)) (PreH4 : (0 <= i)) (PreH5 : (i <= n)) (PreH6 : (n = (string_length (str_l)))) (PreH7 : (cap = (n + 1 ))) (PreH8 : (out <> 0)) (PreH9 : (data <> 0)) (PreH10 : (0 <= out_size)) (PreH11 : (out_size <= i)) (PreH12 : (out_size = (Zlength (output_l)))) (PreH13 : (0 <= level)) (PreH14 : (level <= i)) (PreH15 : (0 <= max_level)) (PreH16 : (max_level <= i)) (PreH17 : (0 <= ch)) (PreH18 : (ch <= 127)) (PreH19 : (valid_string str_l )) (PreH20 : (all_ascii str_l )) (PreH21 : (valid_paren_depth_input_6 str_l )) (PreH22 : (parse_safe_input_6 str_l )) (PreH23 : (((string_length (str_l)) + 1 ) < INT_MAX)) (PreH24 : (problem_6_pre_z str_l )) (PreH25 : (parse_state_6 str_l i level max_level output_l )) ,
+  ((( &( "i" ) )) # Int  |-> i)
+  **  ((( &( "n" ) )) # Int  |-> n)
+  **  ((( &( "cap" ) )) # Int  |-> cap)
+  **  ((( &( "paren_string" ) )) # Ptr  |-> paren_string_pre)
+  **  ((( &( "out" ) )) # Ptr  |-> out)
+  **  ((( &( "data" ) )) # Ptr  |-> data)
+  **  ((( &( "out_size" ) )) # Int  |-> out_size)
+  **  ((( &( "level" ) )) # Int  |-> (level - 1 ))
+  **  ((( &( "max_level" ) )) # Int  |-> max_level)
+  **  ((( &( "ch" ) )) # Int  |-> (Znth i (c_string (str_l)) 0))
+  **  (store_string paren_string_pre str_l )
+  **  ((&((out)  # "<anonymous struct>" ->ₛ "data")) # Ptr  |->_)
+  **  ((&((out)  # "<anonymous struct>" ->ₛ "size")) # Int  |->_)
+  **  (IntArray.seg data 0 out_size output_l )
+  **  (IntArray.undef_seg data out_size cap )
+|--
+  “ (0 <= INT_MAX) ” 
+  &&  “ ((INT_MIN) <= 0) ”
+.
+
+Definition parse_nested_parens_safety_wit_15 := 
+forall (paren_string_pre: Z) (str_l: (@list Z)) (ch: Z) (max_level: Z) (level: Z) (output_l: (@list Z)) (out_size: Z) (data: Z) (out: Z) (cap: Z) (n: Z) (i: Z) (PreH1 : (0 <= ((string_length (str_l)) + 1 ))) (PreH2 : ((level - 1 ) = 0)) (PreH3 : ((Znth i (c_string (str_l)) 0) = 41)) (PreH4 : ((Znth i (c_string (str_l)) 0) <> 40)) (PreH5 : (i < n)) (PreH6 : (0 <= i)) (PreH7 : (i <= n)) (PreH8 : (n = (string_length (str_l)))) (PreH9 : (cap = (n + 1 ))) (PreH10 : (out <> 0)) (PreH11 : (data <> 0)) (PreH12 : (0 <= out_size)) (PreH13 : (out_size <= i)) (PreH14 : (out_size = (Zlength (output_l)))) (PreH15 : (0 <= level)) (PreH16 : (level <= i)) (PreH17 : (0 <= max_level)) (PreH18 : (max_level <= i)) (PreH19 : (0 <= ch)) (PreH20 : (ch <= 127)) (PreH21 : (valid_string str_l )) (PreH22 : (all_ascii str_l )) (PreH23 : (valid_paren_depth_input_6 str_l )) (PreH24 : (parse_safe_input_6 str_l )) (PreH25 : (((string_length (str_l)) + 1 ) < INT_MAX)) (PreH26 : (problem_6_pre_z str_l )) (PreH27 : (parse_state_6 str_l i level max_level output_l )) ,
+  (IntArray.seg data 0 (out_size + 1 ) (app (output_l) ((cons (max_level) ((@nil Z))))) )
+  **  (CharArray.full paren_string_pre ((string_length (str_l)) + 1 ) (c_string (str_l)) )
+  **  (IntArray.undef_seg data (out_size + 1 ) cap )
+  **  ((( &( "i" ) )) # Int  |-> i)
+  **  ((( &( "n" ) )) # Int  |-> n)
+  **  ((( &( "cap" ) )) # Int  |-> cap)
+  **  ((( &( "paren_string" ) )) # Ptr  |-> paren_string_pre)
+  **  ((( &( "out" ) )) # Ptr  |-> out)
+  **  ((( &( "data" ) )) # Ptr  |-> data)
+  **  ((( &( "out_size" ) )) # Int  |-> out_size)
+  **  ((( &( "level" ) )) # Int  |-> (level - 1 ))
+  **  ((( &( "max_level" ) )) # Int  |-> max_level)
+  **  ((( &( "ch" ) )) # Int  |-> (Znth i (c_string (str_l)) 0))
+  **  ((&((out)  # "<anonymous struct>" ->ₛ "data")) # Ptr  |->_)
+  **  ((&((out)  # "<anonymous struct>" ->ₛ "size")) # Int  |->_)
+|--
+  “ ((out_size + 1 ) <= INT_MAX) ” 
+  &&  “ ((INT_MIN) <= (out_size + 1 )) ”
+.
+
+Definition parse_nested_parens_safety_wit_16 := 
+forall (paren_string_pre: Z) (str_l: (@list Z)) (ch: Z) (max_level: Z) (level: Z) (output_l: (@list Z)) (out_size: Z) (data: Z) (out: Z) (cap: Z) (n: Z) (i: Z) (PreH1 : (0 <= ((string_length (str_l)) + 1 ))) (PreH2 : ((level - 1 ) = 0)) (PreH3 : ((Znth i (c_string (str_l)) 0) = 41)) (PreH4 : ((Znth i (c_string (str_l)) 0) <> 40)) (PreH5 : (i < n)) (PreH6 : (0 <= i)) (PreH7 : (i <= n)) (PreH8 : (n = (string_length (str_l)))) (PreH9 : (cap = (n + 1 ))) (PreH10 : (out <> 0)) (PreH11 : (data <> 0)) (PreH12 : (0 <= out_size)) (PreH13 : (out_size <= i)) (PreH14 : (out_size = (Zlength (output_l)))) (PreH15 : (0 <= level)) (PreH16 : (level <= i)) (PreH17 : (0 <= max_level)) (PreH18 : (max_level <= i)) (PreH19 : (0 <= ch)) (PreH20 : (ch <= 127)) (PreH21 : (valid_string str_l )) (PreH22 : (all_ascii str_l )) (PreH23 : (valid_paren_depth_input_6 str_l )) (PreH24 : (parse_safe_input_6 str_l )) (PreH25 : (((string_length (str_l)) + 1 ) < INT_MAX)) (PreH26 : (problem_6_pre_z str_l )) (PreH27 : (parse_state_6 str_l i level max_level output_l )) ,
+  (IntArray.seg data 0 (out_size + 1 ) (app (output_l) ((cons (max_level) ((@nil Z))))) )
+  **  (CharArray.full paren_string_pre ((string_length (str_l)) + 1 ) (c_string (str_l)) )
+  **  (IntArray.undef_seg data (out_size + 1 ) cap )
+  **  ((( &( "i" ) )) # Int  |-> i)
+  **  ((( &( "n" ) )) # Int  |-> n)
+  **  ((( &( "cap" ) )) # Int  |-> cap)
+  **  ((( &( "paren_string" ) )) # Ptr  |-> paren_string_pre)
+  **  ((( &( "out" ) )) # Ptr  |-> out)
+  **  ((( &( "data" ) )) # Ptr  |-> data)
+  **  ((( &( "out_size" ) )) # Int  |-> out_size)
+  **  ((( &( "level" ) )) # Int  |-> (level - 1 ))
+  **  ((( &( "max_level" ) )) # Int  |-> max_level)
+  **  ((( &( "ch" ) )) # Int  |-> (Znth i (c_string (str_l)) 0))
+  **  ((&((out)  # "<anonymous struct>" ->ₛ "data")) # Ptr  |->_)
+  **  ((&((out)  # "<anonymous struct>" ->ₛ "size")) # Int  |->_)
+|--
+  “ (1 <= INT_MAX) ” 
+  &&  “ ((INT_MIN) <= 1) ”
+.
+
+Definition parse_nested_parens_safety_wit_17 := 
+forall (paren_string_pre: Z) (str_l: (@list Z)) (ch: Z) (max_level: Z) (level: Z) (output_l: (@list Z)) (out_size: Z) (data: Z) (out: Z) (cap: Z) (n: Z) (i: Z) (PreH1 : (0 <= ((string_length (str_l)) + 1 ))) (PreH2 : ((level - 1 ) = 0)) (PreH3 : ((Znth i (c_string (str_l)) 0) = 41)) (PreH4 : ((Znth i (c_string (str_l)) 0) <> 40)) (PreH5 : (i < n)) (PreH6 : (0 <= i)) (PreH7 : (i <= n)) (PreH8 : (n = (string_length (str_l)))) (PreH9 : (cap = (n + 1 ))) (PreH10 : (out <> 0)) (PreH11 : (data <> 0)) (PreH12 : (0 <= out_size)) (PreH13 : (out_size <= i)) (PreH14 : (out_size = (Zlength (output_l)))) (PreH15 : (0 <= level)) (PreH16 : (level <= i)) (PreH17 : (0 <= max_level)) (PreH18 : (max_level <= i)) (PreH19 : (0 <= ch)) (PreH20 : (ch <= 127)) (PreH21 : (valid_string str_l )) (PreH22 : (all_ascii str_l )) (PreH23 : (valid_paren_depth_input_6 str_l )) (PreH24 : (parse_safe_input_6 str_l )) (PreH25 : (((string_length (str_l)) + 1 ) < INT_MAX)) (PreH26 : (problem_6_pre_z str_l )) (PreH27 : (parse_state_6 str_l i level max_level output_l )) ,
+  (IntArray.seg data 0 (out_size + 1 ) (app (output_l) ((cons (max_level) ((@nil Z))))) )
+  **  (CharArray.full paren_string_pre ((string_length (str_l)) + 1 ) (c_string (str_l)) )
+  **  (IntArray.undef_seg data (out_size + 1 ) cap )
+  **  ((( &( "i" ) )) # Int  |-> i)
+  **  ((( &( "n" ) )) # Int  |-> n)
+  **  ((( &( "cap" ) )) # Int  |-> cap)
+  **  ((( &( "paren_string" ) )) # Ptr  |-> paren_string_pre)
+  **  ((( &( "out" ) )) # Ptr  |-> out)
+  **  ((( &( "data" ) )) # Ptr  |-> data)
+  **  ((( &( "out_size" ) )) # Int  |-> (out_size + 1 ))
+  **  ((( &( "level" ) )) # Int  |-> (level - 1 ))
+  **  ((( &( "max_level" ) )) # Int  |-> max_level)
+  **  ((( &( "ch" ) )) # Int  |-> (Znth i (c_string (str_l)) 0))
+  **  ((&((out)  # "<anonymous struct>" ->ₛ "data")) # Ptr  |->_)
+  **  ((&((out)  # "<anonymous struct>" ->ₛ "size")) # Int  |->_)
+|--
+  “ (0 <= INT_MAX) ” 
+  &&  “ ((INT_MIN) <= 0) ”
+.
+
+Definition parse_nested_parens_safety_wit_18 := 
+forall (paren_string_pre: Z) (str_l: (@list Z)) (output_l: (@list Z)) (i: Z) (n: Z) (cap: Z) (out: Z) (data: Z) (ch: Z) (out_size: Z) (level: Z) (max_level: Z) (PreH1 : (0 <= i)) (PreH2 : (i < n)) (PreH3 : (n = (string_length (str_l)))) (PreH4 : (cap = (n + 1 ))) (PreH5 : (out <> 0)) (PreH6 : (data <> 0)) (PreH7 : (ch = 40)) (PreH8 : (0 <= out_size)) (PreH9 : (out_size <= i)) (PreH10 : (out_size = (Zlength (output_l)))) (PreH11 : (1 <= level)) (PreH12 : (level <= (i + 1 ))) (PreH13 : (1 <= max_level)) (PreH14 : (max_level <= (i + 1 ))) (PreH15 : (valid_string str_l )) (PreH16 : (all_ascii str_l )) (PreH17 : (valid_paren_depth_input_6 str_l )) (PreH18 : (parse_safe_input_6 str_l )) (PreH19 : (((string_length (str_l)) + 1 ) < INT_MAX)) (PreH20 : (problem_6_pre_z str_l )) (PreH21 : (parse_state_6 str_l (i + 1 ) level max_level output_l )) ,
+  ((( &( "i" ) )) # Int  |-> i)
+  **  ((( &( "n" ) )) # Int  |-> n)
+  **  ((( &( "cap" ) )) # Int  |-> cap)
+  **  ((( &( "paren_string" ) )) # Ptr  |-> paren_string_pre)
+  **  ((( &( "out" ) )) # Ptr  |-> out)
+  **  ((( &( "data" ) )) # Ptr  |-> data)
+  **  ((( &( "ch" ) )) # Int  |-> ch)
+  **  ((( &( "out_size" ) )) # Int  |-> out_size)
+  **  ((( &( "level" ) )) # Int  |-> level)
+  **  ((( &( "max_level" ) )) # Int  |-> max_level)
+  **  (store_string paren_string_pre str_l )
+  **  ((&((out)  # "<anonymous struct>" ->ₛ "data")) # Ptr  |->_)
+  **  ((&((out)  # "<anonymous struct>" ->ₛ "size")) # Int  |->_)
+  **  (IntArray.seg data 0 out_size output_l )
+  **  (IntArray.undef_seg data out_size cap )
+|--
+  “ ((i + 1 ) <= INT_MAX) ” 
+  &&  “ ((INT_MIN) <= (i + 1 )) ”
+.
+
+Definition parse_nested_parens_safety_wit_19 := 
+forall (paren_string_pre: Z) (str_l: (@list Z)) (output_l: (@list Z)) (i: Z) (n: Z) (cap: Z) (out: Z) (data: Z) (ch: Z) (out_size: Z) (level: Z) (max_level: Z) (PreH1 : (0 <= i)) (PreH2 : (i < n)) (PreH3 : (n = (string_length (str_l)))) (PreH4 : (cap = (n + 1 ))) (PreH5 : (out <> 0)) (PreH6 : (data <> 0)) (PreH7 : (ch = 41)) (PreH8 : (1 <= out_size)) (PreH9 : (out_size <= (i + 1 ))) (PreH10 : (out_size = (Zlength (output_l)))) (PreH11 : (level = 0)) (PreH12 : (max_level = 0)) (PreH13 : (valid_string str_l )) (PreH14 : (all_ascii str_l )) (PreH15 : (valid_paren_depth_input_6 str_l )) (PreH16 : (parse_safe_input_6 str_l )) (PreH17 : (((string_length (str_l)) + 1 ) < INT_MAX)) (PreH18 : (problem_6_pre_z str_l )) (PreH19 : (parse_state_6 str_l (i + 1 ) level max_level output_l )) ,
+  ((( &( "i" ) )) # Int  |-> i)
+  **  ((( &( "n" ) )) # Int  |-> n)
+  **  ((( &( "cap" ) )) # Int  |-> cap)
+  **  ((( &( "paren_string" ) )) # Ptr  |-> paren_string_pre)
+  **  ((( &( "out" ) )) # Ptr  |-> out)
+  **  ((( &( "data" ) )) # Ptr  |-> data)
+  **  ((( &( "ch" ) )) # Int  |-> ch)
+  **  ((( &( "out_size" ) )) # Int  |-> out_size)
+  **  ((( &( "level" ) )) # Int  |-> level)
+  **  ((( &( "max_level" ) )) # Int  |-> max_level)
+  **  (store_string paren_string_pre str_l )
+  **  ((&((out)  # "<anonymous struct>" ->ₛ "data")) # Ptr  |->_)
+  **  ((&((out)  # "<anonymous struct>" ->ₛ "size")) # Int  |->_)
+  **  (IntArray.seg data 0 out_size output_l )
+  **  (IntArray.undef_seg data out_size cap )
+|--
+  “ ((i + 1 ) <= INT_MAX) ” 
+  &&  “ ((INT_MIN) <= (i + 1 )) ”
+.
+
+Definition parse_nested_parens_safety_wit_20 := 
+forall (paren_string_pre: Z) (str_l: (@list Z)) (output_l: (@list Z)) (i: Z) (n: Z) (cap: Z) (out: Z) (data: Z) (ch: Z) (out_size: Z) (level: Z) (max_level: Z) (PreH1 : (0 <= i)) (PreH2 : (i < n)) (PreH3 : (n = (string_length (str_l)))) (PreH4 : (cap = (n + 1 ))) (PreH5 : (out <> 0)) (PreH6 : (data <> 0)) (PreH7 : (ch = 41)) (PreH8 : (0 <= out_size)) (PreH9 : (out_size <= i)) (PreH10 : (out_size = (Zlength (output_l)))) (PreH11 : (0 < level)) (PreH12 : (level <= i)) (PreH13 : (0 <= max_level)) (PreH14 : (max_level <= i)) (PreH15 : (valid_string str_l )) (PreH16 : (all_ascii str_l )) (PreH17 : (valid_paren_depth_input_6 str_l )) (PreH18 : (parse_safe_input_6 str_l )) (PreH19 : (((string_length (str_l)) + 1 ) < INT_MAX)) (PreH20 : (problem_6_pre_z str_l )) (PreH21 : (parse_state_6 str_l (i + 1 ) level max_level output_l )) ,
+  ((( &( "i" ) )) # Int  |-> i)
+  **  ((( &( "n" ) )) # Int  |-> n)
+  **  ((( &( "cap" ) )) # Int  |-> cap)
+  **  ((( &( "paren_string" ) )) # Ptr  |-> paren_string_pre)
+  **  ((( &( "out" ) )) # Ptr  |-> out)
+  **  ((( &( "data" ) )) # Ptr  |-> data)
+  **  ((( &( "ch" ) )) # Int  |-> ch)
+  **  ((( &( "out_size" ) )) # Int  |-> out_size)
+  **  ((( &( "level" ) )) # Int  |-> level)
+  **  ((( &( "max_level" ) )) # Int  |-> max_level)
+  **  (store_string paren_string_pre str_l )
+  **  ((&((out)  # "<anonymous struct>" ->ₛ "data")) # Ptr  |->_)
+  **  ((&((out)  # "<anonymous struct>" ->ₛ "size")) # Int  |->_)
+  **  (IntArray.seg data 0 out_size output_l )
+  **  (IntArray.undef_seg data out_size cap )
+|--
+  “ ((i + 1 ) <= INT_MAX) ” 
+  &&  “ ((INT_MIN) <= (i + 1 )) ”
+.
+
+Definition parse_nested_parens_safety_wit_21 := 
+forall (paren_string_pre: Z) (str_l: (@list Z)) (output_l: (@list Z)) (i: Z) (n: Z) (cap: Z) (out: Z) (data: Z) (ch: Z) (out_size: Z) (level: Z) (max_level: Z) (PreH1 : (0 <= i)) (PreH2 : (i < n)) (PreH3 : (n = (string_length (str_l)))) (PreH4 : (cap = (n + 1 ))) (PreH5 : (out <> 0)) (PreH6 : (data <> 0)) (PreH7 : (ch = 32)) (PreH8 : (0 <= out_size)) (PreH9 : (out_size <= i)) (PreH10 : (out_size = (Zlength (output_l)))) (PreH11 : (0 <= level)) (PreH12 : (level <= i)) (PreH13 : (0 <= max_level)) (PreH14 : (max_level <= i)) (PreH15 : (valid_string str_l )) (PreH16 : (all_ascii str_l )) (PreH17 : (valid_paren_depth_input_6 str_l )) (PreH18 : (parse_safe_input_6 str_l )) (PreH19 : (((string_length (str_l)) + 1 ) < INT_MAX)) (PreH20 : (problem_6_pre_z str_l )) (PreH21 : (parse_state_6 str_l (i + 1 ) level max_level output_l )) ,
+  ((( &( "i" ) )) # Int  |-> i)
+  **  ((( &( "n" ) )) # Int  |-> n)
+  **  ((( &( "cap" ) )) # Int  |-> cap)
+  **  ((( &( "paren_string" ) )) # Ptr  |-> paren_string_pre)
+  **  ((( &( "out" ) )) # Ptr  |-> out)
+  **  ((( &( "data" ) )) # Ptr  |-> data)
+  **  ((( &( "ch" ) )) # Int  |-> ch)
+  **  ((( &( "out_size" ) )) # Int  |-> out_size)
+  **  ((( &( "level" ) )) # Int  |-> level)
+  **  ((( &( "max_level" ) )) # Int  |-> max_level)
+  **  (store_string paren_string_pre str_l )
+  **  ((&((out)  # "<anonymous struct>" ->ₛ "data")) # Ptr  |->_)
+  **  ((&((out)  # "<anonymous struct>" ->ₛ "size")) # Int  |->_)
+  **  (IntArray.seg data 0 out_size output_l )
+  **  (IntArray.undef_seg data out_size cap )
+|--
+  “ ((i + 1 ) <= INT_MAX) ” 
+  &&  “ ((INT_MIN) <= (i + 1 )) ”
+.
+
+Definition parse_nested_parens_entail_wit_1 := 
+(
+forall (paren_string_pre: Z) (str_l: (@list Z)) (retval: Z) (retval_2: Z) (retval_3: Z) (PreH1 : (retval_3 <> 0)) (PreH2 : (retval_2 <> 0)) (PreH3 : (retval = (string_length (str_l)))) (PreH4 : (0 <= ((string_length (str_l)) + 1 ))) (PreH5 : (valid_string str_l )) (PreH6 : (all_ascii str_l )) (PreH7 : (valid_paren_depth_input_6 str_l )) (PreH8 : (parse_safe_input_6 str_l )) (PreH9 : (((string_length (str_l)) + 1 ) < INT_MAX)) (PreH10 : (problem_6_pre_z str_l )) ,
+  (IntArray.undef_full retval_3 (retval + 1 ) )
+  **  ((&((retval_2)  # "<anonymous struct>" ->ₛ "data")) # Ptr  |->_)
+  **  ((&((retval_2)  # "<anonymous struct>" ->ₛ "size")) # Int  |->_)
+  **  (CharArray.full paren_string_pre ((string_length (str_l)) + 1 ) (c_string (str_l)) )
+|--
+  EX (output_l: (@list Z)) ,
+  “ (0 <= 0) ” 
+  &&  “ (0 <= retval) ” 
+  &&  “ (retval = (string_length (str_l))) ” 
+  &&  “ ((retval + 1 ) = (retval + 1 )) ” 
+  &&  “ (retval_2 <> 0) ” 
+  &&  “ (retval_3 <> 0) ” 
+  &&  “ (0 <= 0) ” 
+  &&  “ (0 <= 0) ” 
+  &&  “ (0 = (Zlength (output_l))) ” 
+  &&  “ (0 <= 0) ” 
+  &&  “ (0 <= 0) ” 
+  &&  “ (0 <= 0) ” 
+  &&  “ (0 <= 0) ” 
+  &&  “ (0 <= 0) ” 
+  &&  “ (0 <= 127) ” 
+  &&  “ (valid_string str_l ) ” 
+  &&  “ (all_ascii str_l ) ” 
+  &&  “ (valid_paren_depth_input_6 str_l ) ” 
+  &&  “ (parse_safe_input_6 str_l ) ” 
+  &&  “ (((string_length (str_l)) + 1 ) < INT_MAX) ” 
+  &&  “ (problem_6_pre_z str_l ) ” 
+  &&  “ (parse_state_6 str_l 0 0 0 output_l ) ”
+  &&  (store_string paren_string_pre str_l )
+  **  ((&((retval_2)  # "<anonymous struct>" ->ₛ "data")) # Ptr  |->_)
+  **  ((&((retval_2)  # "<anonymous struct>" ->ₛ "size")) # Int  |->_)
+  **  (IntArray.seg retval_3 0 0 output_l )
+  **  (IntArray.undef_seg retval_3 0 (retval + 1 ) )
+) \/
+(
+forall (str_l: (@list Z)) (retval: Z) (retval_2: Z) (retval_3: Z) (PreH1 : (retval_3 <> 0)) (PreH2 : (retval_2 <> 0)) (PreH3 : (retval = (string_length (str_l)))) (PreH4 : (0 <= ((string_length (str_l)) + 1 ))) (PreH5 : (valid_string str_l )) (PreH6 : (all_ascii str_l )) (PreH7 : (valid_paren_depth_input_6 str_l )) (PreH8 : (parse_safe_input_6 str_l )) (PreH9 : (((string_length (str_l)) + 1 ) < INT_MAX)) (PreH10 : (problem_6_pre_z str_l )) ,
+  TT && emp 
+|--
+  “ (parse_state_6 str_l 0 0 0 (@nil Z) ) ” 
+  &&  “ (0 = (Zlength ((@nil Z)))) ” 
+  &&  “ (0 <= retval) ”
+  &&  emp
+).
+
+Definition parse_nested_parens_entail_wit_1_split_goal_1 := 
+forall (str_l: (@list Z)) (retval: Z) (retval_2: Z) (retval_3: Z) (PreH1 : (retval_3 <> 0)) (PreH2 : (retval_2 <> 0)) (PreH3 : (retval = (string_length (str_l)))) (PreH4 : (0 <= ((string_length (str_l)) + 1 ))) (PreH5 : (valid_string str_l )) (PreH6 : (all_ascii str_l )) (PreH7 : (valid_paren_depth_input_6 str_l )) (PreH8 : (parse_safe_input_6 str_l )) (PreH9 : (((string_length (str_l)) + 1 ) < INT_MAX)) (PreH10 : (problem_6_pre_z str_l )) ,
+  TT && emp 
+|--
+  “ (parse_state_6 str_l 0 0 0 (@nil Z) ) ”
+.
+
+Definition parse_nested_parens_entail_wit_1_split_goal_2 := 
+forall (str_l: (@list Z)) (retval: Z) (retval_2: Z) (retval_3: Z) (PreH1 : (retval_3 <> 0)) (PreH2 : (retval_2 <> 0)) (PreH3 : (retval = (string_length (str_l)))) (PreH4 : (0 <= ((string_length (str_l)) + 1 ))) (PreH5 : (valid_string str_l )) (PreH6 : (all_ascii str_l )) (PreH7 : (valid_paren_depth_input_6 str_l )) (PreH8 : (parse_safe_input_6 str_l )) (PreH9 : (((string_length (str_l)) + 1 ) < INT_MAX)) (PreH10 : (problem_6_pre_z str_l )) ,
+  TT && emp 
+|--
+  “ (0 = (Zlength ((@nil Z)))) ”
+.
+
+Definition parse_nested_parens_entail_wit_1_split_goal_3 := 
+forall (str_l: (@list Z)) (retval: Z) (retval_2: Z) (retval_3: Z) (PreH1 : (retval_3 <> 0)) (PreH2 : (retval_2 <> 0)) (PreH3 : (retval = (string_length (str_l)))) (PreH4 : (0 <= ((string_length (str_l)) + 1 ))) (PreH5 : (valid_string str_l )) (PreH6 : (all_ascii str_l )) (PreH7 : (valid_paren_depth_input_6 str_l )) (PreH8 : (parse_safe_input_6 str_l )) (PreH9 : (((string_length (str_l)) + 1 ) < INT_MAX)) (PreH10 : (problem_6_pre_z str_l )) ,
+  TT && emp 
+|--
+  “ (0 <= retval) ”
+.
+
+Definition parse_nested_parens_entail_wit_2_1 := 
+(
+forall (paren_string_pre: Z) (str_l: (@list Z)) (ch: Z) (max_level: Z) (level: Z) (output_l_2: (@list Z)) (out_size: Z) (data: Z) (out: Z) (cap: Z) (n: Z) (i: Z) (PreH1 : ((level + 1 ) <= max_level)) (PreH2 : ((Znth i (c_string (str_l)) 0) = 40)) (PreH3 : (i < n)) (PreH4 : (0 <= i)) (PreH5 : (i <= n)) (PreH6 : (n = (string_length (str_l)))) (PreH7 : (cap = (n + 1 ))) (PreH8 : (out <> 0)) (PreH9 : (data <> 0)) (PreH10 : (0 <= out_size)) (PreH11 : (out_size <= i)) (PreH12 : (out_size = (Zlength (output_l_2)))) (PreH13 : (0 <= level)) (PreH14 : (level <= i)) (PreH15 : (0 <= max_level)) (PreH16 : (max_level <= i)) (PreH17 : (0 <= ch)) (PreH18 : (ch <= 127)) (PreH19 : (valid_string str_l )) (PreH20 : (all_ascii str_l )) (PreH21 : (valid_paren_depth_input_6 str_l )) (PreH22 : (parse_safe_input_6 str_l )) (PreH23 : (((string_length (str_l)) + 1 ) < INT_MAX)) (PreH24 : (problem_6_pre_z str_l )) (PreH25 : (parse_state_6 str_l i level max_level output_l_2 )) ,
+  (store_string paren_string_pre str_l )
+  **  ((&((out)  # "<anonymous struct>" ->ₛ "data")) # Ptr  |->_)
+  **  ((&((out)  # "<anonymous struct>" ->ₛ "size")) # Int  |->_)
+  **  (IntArray.seg data 0 out_size output_l_2 )
+  **  (IntArray.undef_seg data out_size cap )
+|--
+  EX (output_l: (@list Z)) ,
+  “ (0 <= i) ” 
+  &&  “ (i < n) ” 
+  &&  “ (n = (string_length (str_l))) ” 
+  &&  “ (cap = (n + 1 )) ” 
+  &&  “ (out <> 0) ” 
+  &&  “ (data <> 0) ” 
+  &&  “ ((Znth i (c_string (str_l)) 0) = 40) ” 
+  &&  “ (0 <= out_size) ” 
+  &&  “ (out_size <= i) ” 
+  &&  “ (out_size = (Zlength (output_l))) ” 
+  &&  “ (1 <= (level + 1 )) ” 
+  &&  “ ((level + 1 ) <= (i + 1 )) ” 
+  &&  “ (1 <= max_level) ” 
+  &&  “ (max_level <= (i + 1 )) ” 
+  &&  “ (valid_string str_l ) ” 
+  &&  “ (all_ascii str_l ) ” 
+  &&  “ (valid_paren_depth_input_6 str_l ) ” 
+  &&  “ (parse_safe_input_6 str_l ) ” 
+  &&  “ (((string_length (str_l)) + 1 ) < INT_MAX) ” 
+  &&  “ (problem_6_pre_z str_l ) ” 
+  &&  “ (parse_state_6 str_l (i + 1 ) (level + 1 ) max_level output_l ) ”
+  &&  (store_string paren_string_pre str_l )
+  **  ((&((out)  # "<anonymous struct>" ->ₛ "data")) # Ptr  |->_)
+  **  ((&((out)  # "<anonymous struct>" ->ₛ "size")) # Int  |->_)
+  **  (IntArray.seg data 0 out_size output_l )
+  **  (IntArray.undef_seg data out_size cap )
+) \/
+(
+forall (str_l: (@list Z)) (ch: Z) (max_level: Z) (level: Z) (output_l_2: (@list Z)) (out_size: Z) (data: Z) (out: Z) (cap: Z) (n: Z) (i: Z) (PreH1 : (0 <= ((string_length (str_l)) + 1 ))) (PreH2 : ((level + 1 ) <= max_level)) (PreH3 : ((Znth i (c_string (str_l)) 0) = 40)) (PreH4 : (i < n)) (PreH5 : (0 <= i)) (PreH6 : (i <= n)) (PreH7 : (n = (string_length (str_l)))) (PreH8 : (cap = (n + 1 ))) (PreH9 : (out <> 0)) (PreH10 : (data <> 0)) (PreH11 : (0 <= out_size)) (PreH12 : (out_size <= i)) (PreH13 : (out_size = (Zlength (output_l_2)))) (PreH14 : (0 <= level)) (PreH15 : (level <= i)) (PreH16 : (0 <= max_level)) (PreH17 : (max_level <= i)) (PreH18 : (0 <= ch)) (PreH19 : (ch <= 127)) (PreH20 : (valid_string str_l )) (PreH21 : (all_ascii str_l )) (PreH22 : (valid_paren_depth_input_6 str_l )) (PreH23 : (parse_safe_input_6 str_l )) (PreH24 : (((string_length (str_l)) + 1 ) < INT_MAX)) (PreH25 : (problem_6_pre_z str_l )) (PreH26 : (parse_state_6 str_l i level max_level output_l_2 )) ,
+  TT && emp 
+|--
+  “ (parse_state_6 str_l (i + 1 ) (level + 1 ) max_level output_l_2 ) ”
+  &&  emp
+).
+
+Definition parse_nested_parens_entail_wit_2_1_split_goal_1 := 
+forall (str_l: (@list Z)) (ch: Z) (max_level: Z) (level: Z) (output_l_2: (@list Z)) (out_size: Z) (data: Z) (out: Z) (cap: Z) (n: Z) (i: Z) (PreH1 : (0 <= ((string_length (str_l)) + 1 ))) (PreH2 : ((level + 1 ) <= max_level)) (PreH3 : ((Znth i (c_string (str_l)) 0) = 40)) (PreH4 : (i < n)) (PreH5 : (0 <= i)) (PreH6 : (i <= n)) (PreH7 : (n = (string_length (str_l)))) (PreH8 : (cap = (n + 1 ))) (PreH9 : (out <> 0)) (PreH10 : (data <> 0)) (PreH11 : (0 <= out_size)) (PreH12 : (out_size <= i)) (PreH13 : (out_size = (Zlength (output_l_2)))) (PreH14 : (0 <= level)) (PreH15 : (level <= i)) (PreH16 : (0 <= max_level)) (PreH17 : (max_level <= i)) (PreH18 : (0 <= ch)) (PreH19 : (ch <= 127)) (PreH20 : (valid_string str_l )) (PreH21 : (all_ascii str_l )) (PreH22 : (valid_paren_depth_input_6 str_l )) (PreH23 : (parse_safe_input_6 str_l )) (PreH24 : (((string_length (str_l)) + 1 ) < INT_MAX)) (PreH25 : (problem_6_pre_z str_l )) (PreH26 : (parse_state_6 str_l i level max_level output_l_2 )) ,
+  TT && emp 
+|--
+  “ (parse_state_6 str_l (i + 1 ) (level + 1 ) max_level output_l_2 ) ”
+.
+
+Definition parse_nested_parens_entail_wit_2_2 := 
+(
+forall (paren_string_pre: Z) (str_l: (@list Z)) (ch: Z) (max_level: Z) (level: Z) (output_l_2: (@list Z)) (out_size: Z) (data: Z) (out: Z) (cap: Z) (n: Z) (i: Z) (PreH1 : ((level + 1 ) > max_level)) (PreH2 : ((Znth i (c_string (str_l)) 0) = 40)) (PreH3 : (i < n)) (PreH4 : (0 <= i)) (PreH5 : (i <= n)) (PreH6 : (n = (string_length (str_l)))) (PreH7 : (cap = (n + 1 ))) (PreH8 : (out <> 0)) (PreH9 : (data <> 0)) (PreH10 : (0 <= out_size)) (PreH11 : (out_size <= i)) (PreH12 : (out_size = (Zlength (output_l_2)))) (PreH13 : (0 <= level)) (PreH14 : (level <= i)) (PreH15 : (0 <= max_level)) (PreH16 : (max_level <= i)) (PreH17 : (0 <= ch)) (PreH18 : (ch <= 127)) (PreH19 : (valid_string str_l )) (PreH20 : (all_ascii str_l )) (PreH21 : (valid_paren_depth_input_6 str_l )) (PreH22 : (parse_safe_input_6 str_l )) (PreH23 : (((string_length (str_l)) + 1 ) < INT_MAX)) (PreH24 : (problem_6_pre_z str_l )) (PreH25 : (parse_state_6 str_l i level max_level output_l_2 )) ,
+  (store_string paren_string_pre str_l )
+  **  ((&((out)  # "<anonymous struct>" ->ₛ "data")) # Ptr  |->_)
+  **  ((&((out)  # "<anonymous struct>" ->ₛ "size")) # Int  |->_)
+  **  (IntArray.seg data 0 out_size output_l_2 )
+  **  (IntArray.undef_seg data out_size cap )
+|--
+  EX (output_l: (@list Z)) ,
+  “ (0 <= i) ” 
+  &&  “ (i < n) ” 
+  &&  “ (n = (string_length (str_l))) ” 
+  &&  “ (cap = (n + 1 )) ” 
+  &&  “ (out <> 0) ” 
+  &&  “ (data <> 0) ” 
+  &&  “ ((Znth i (c_string (str_l)) 0) = 40) ” 
+  &&  “ (0 <= out_size) ” 
+  &&  “ (out_size <= i) ” 
+  &&  “ (out_size = (Zlength (output_l))) ” 
+  &&  “ (1 <= (level + 1 )) ” 
+  &&  “ ((level + 1 ) <= (i + 1 )) ” 
+  &&  “ (1 <= (level + 1 )) ” 
+  &&  “ ((level + 1 ) <= (i + 1 )) ” 
+  &&  “ (valid_string str_l ) ” 
+  &&  “ (all_ascii str_l ) ” 
+  &&  “ (valid_paren_depth_input_6 str_l ) ” 
+  &&  “ (parse_safe_input_6 str_l ) ” 
+  &&  “ (((string_length (str_l)) + 1 ) < INT_MAX) ” 
+  &&  “ (problem_6_pre_z str_l ) ” 
+  &&  “ (parse_state_6 str_l (i + 1 ) (level + 1 ) (level + 1 ) output_l ) ”
+  &&  (store_string paren_string_pre str_l )
+  **  ((&((out)  # "<anonymous struct>" ->ₛ "data")) # Ptr  |->_)
+  **  ((&((out)  # "<anonymous struct>" ->ₛ "size")) # Int  |->_)
+  **  (IntArray.seg data 0 out_size output_l )
+  **  (IntArray.undef_seg data out_size cap )
+) \/
+(
+forall (str_l: (@list Z)) (ch: Z) (max_level: Z) (level: Z) (output_l_2: (@list Z)) (out_size: Z) (data: Z) (out: Z) (cap: Z) (n: Z) (i: Z) (PreH1 : (0 <= ((string_length (str_l)) + 1 ))) (PreH2 : ((level + 1 ) > max_level)) (PreH3 : ((Znth i (c_string (str_l)) 0) = 40)) (PreH4 : (i < n)) (PreH5 : (0 <= i)) (PreH6 : (i <= n)) (PreH7 : (n = (string_length (str_l)))) (PreH8 : (cap = (n + 1 ))) (PreH9 : (out <> 0)) (PreH10 : (data <> 0)) (PreH11 : (0 <= out_size)) (PreH12 : (out_size <= i)) (PreH13 : (out_size = (Zlength (output_l_2)))) (PreH14 : (0 <= level)) (PreH15 : (level <= i)) (PreH16 : (0 <= max_level)) (PreH17 : (max_level <= i)) (PreH18 : (0 <= ch)) (PreH19 : (ch <= 127)) (PreH20 : (valid_string str_l )) (PreH21 : (all_ascii str_l )) (PreH22 : (valid_paren_depth_input_6 str_l )) (PreH23 : (parse_safe_input_6 str_l )) (PreH24 : (((string_length (str_l)) + 1 ) < INT_MAX)) (PreH25 : (problem_6_pre_z str_l )) (PreH26 : (parse_state_6 str_l i level max_level output_l_2 )) ,
+  TT && emp 
+|--
+  “ (parse_state_6 str_l (i + 1 ) (level + 1 ) (level + 1 ) output_l_2 ) ”
+  &&  emp
+).
+
+Definition parse_nested_parens_entail_wit_2_2_split_goal_1 := 
+forall (str_l: (@list Z)) (ch: Z) (max_level: Z) (level: Z) (output_l_2: (@list Z)) (out_size: Z) (data: Z) (out: Z) (cap: Z) (n: Z) (i: Z) (PreH1 : (0 <= ((string_length (str_l)) + 1 ))) (PreH2 : ((level + 1 ) > max_level)) (PreH3 : ((Znth i (c_string (str_l)) 0) = 40)) (PreH4 : (i < n)) (PreH5 : (0 <= i)) (PreH6 : (i <= n)) (PreH7 : (n = (string_length (str_l)))) (PreH8 : (cap = (n + 1 ))) (PreH9 : (out <> 0)) (PreH10 : (data <> 0)) (PreH11 : (0 <= out_size)) (PreH12 : (out_size <= i)) (PreH13 : (out_size = (Zlength (output_l_2)))) (PreH14 : (0 <= level)) (PreH15 : (level <= i)) (PreH16 : (0 <= max_level)) (PreH17 : (max_level <= i)) (PreH18 : (0 <= ch)) (PreH19 : (ch <= 127)) (PreH20 : (valid_string str_l )) (PreH21 : (all_ascii str_l )) (PreH22 : (valid_paren_depth_input_6 str_l )) (PreH23 : (parse_safe_input_6 str_l )) (PreH24 : (((string_length (str_l)) + 1 ) < INT_MAX)) (PreH25 : (problem_6_pre_z str_l )) (PreH26 : (parse_state_6 str_l i level max_level output_l_2 )) ,
+  TT && emp 
+|--
+  “ (parse_state_6 str_l (i + 1 ) (level + 1 ) (level + 1 ) output_l_2 ) ”
+.
+
+Definition parse_nested_parens_entail_wit_3 := 
+(
+forall (paren_string_pre: Z) (str_l: (@list Z)) (ch: Z) (max_level: Z) (level: Z) (output_l_2: (@list Z)) (out_size: Z) (data: Z) (out: Z) (cap: Z) (n: Z) (i: Z) (PreH1 : (0 <= ((string_length (str_l)) + 1 ))) (PreH2 : ((level - 1 ) = 0)) (PreH3 : ((Znth i (c_string (str_l)) 0) = 41)) (PreH4 : ((Znth i (c_string (str_l)) 0) <> 40)) (PreH5 : (i < n)) (PreH6 : (0 <= i)) (PreH7 : (i <= n)) (PreH8 : (n = (string_length (str_l)))) (PreH9 : (cap = (n + 1 ))) (PreH10 : (out <> 0)) (PreH11 : (data <> 0)) (PreH12 : (0 <= out_size)) (PreH13 : (out_size <= i)) (PreH14 : (out_size = (Zlength (output_l_2)))) (PreH15 : (0 <= level)) (PreH16 : (level <= i)) (PreH17 : (0 <= max_level)) (PreH18 : (max_level <= i)) (PreH19 : (0 <= ch)) (PreH20 : (ch <= 127)) (PreH21 : (valid_string str_l )) (PreH22 : (all_ascii str_l )) (PreH23 : (valid_paren_depth_input_6 str_l )) (PreH24 : (parse_safe_input_6 str_l )) (PreH25 : (((string_length (str_l)) + 1 ) < INT_MAX)) (PreH26 : (problem_6_pre_z str_l )) (PreH27 : (parse_state_6 str_l i level max_level output_l_2 )) ,
+  (IntArray.seg data 0 (out_size + 1 ) (app (output_l_2) ((cons (max_level) ((@nil Z))))) )
+  **  (CharArray.full paren_string_pre ((string_length (str_l)) + 1 ) (c_string (str_l)) )
+  **  (IntArray.undef_seg data (out_size + 1 ) cap )
+  **  ((&((out)  # "<anonymous struct>" ->ₛ "data")) # Ptr  |->_)
+  **  ((&((out)  # "<anonymous struct>" ->ₛ "size")) # Int  |->_)
+|--
+  EX (output_l: (@list Z)) ,
+  “ (0 <= i) ” 
+  &&  “ (i < n) ” 
+  &&  “ (n = (string_length (str_l))) ” 
+  &&  “ (cap = (n + 1 )) ” 
+  &&  “ (out <> 0) ” 
+  &&  “ (data <> 0) ” 
+  &&  “ ((Znth i (c_string (str_l)) 0) = 41) ” 
+  &&  “ (1 <= (out_size + 1 )) ” 
+  &&  “ ((out_size + 1 ) <= (i + 1 )) ” 
+  &&  “ ((out_size + 1 ) = (Zlength (output_l))) ” 
+  &&  “ ((level - 1 ) = 0) ” 
+  &&  “ (0 = 0) ” 
+  &&  “ (valid_string str_l ) ” 
+  &&  “ (all_ascii str_l ) ” 
+  &&  “ (valid_paren_depth_input_6 str_l ) ” 
+  &&  “ (parse_safe_input_6 str_l ) ” 
+  &&  “ (((string_length (str_l)) + 1 ) < INT_MAX) ” 
+  &&  “ (problem_6_pre_z str_l ) ” 
+  &&  “ (parse_state_6 str_l (i + 1 ) (level - 1 ) 0 output_l ) ”
+  &&  (store_string paren_string_pre str_l )
+  **  ((&((out)  # "<anonymous struct>" ->ₛ "data")) # Ptr  |->_)
+  **  ((&((out)  # "<anonymous struct>" ->ₛ "size")) # Int  |->_)
+  **  (IntArray.seg data 0 (out_size + 1 ) output_l )
+  **  (IntArray.undef_seg data (out_size + 1 ) cap )
+) \/
+(
+forall (str_l: (@list Z)) (ch: Z) (max_level: Z) (level: Z) (output_l_2: (@list Z)) (out_size: Z) (data: Z) (out: Z) (cap: Z) (n: Z) (i: Z) (PreH1 : (0 <= ((string_length (str_l)) + 1 ))) (PreH2 : ((level - 1 ) = 0)) (PreH3 : ((Znth i (c_string (str_l)) 0) = 41)) (PreH4 : ((Znth i (c_string (str_l)) 0) <> 40)) (PreH5 : (i < n)) (PreH6 : (0 <= i)) (PreH7 : (i <= n)) (PreH8 : (n = (string_length (str_l)))) (PreH9 : (cap = (n + 1 ))) (PreH10 : (out <> 0)) (PreH11 : (data <> 0)) (PreH12 : (0 <= out_size)) (PreH13 : (out_size <= i)) (PreH14 : (out_size = (Zlength (output_l_2)))) (PreH15 : (0 <= level)) (PreH16 : (level <= i)) (PreH17 : (0 <= max_level)) (PreH18 : (max_level <= i)) (PreH19 : (0 <= ch)) (PreH20 : (ch <= 127)) (PreH21 : (valid_string str_l )) (PreH22 : (all_ascii str_l )) (PreH23 : (valid_paren_depth_input_6 str_l )) (PreH24 : (parse_safe_input_6 str_l )) (PreH25 : (((string_length (str_l)) + 1 ) < INT_MAX)) (PreH26 : (problem_6_pre_z str_l )) (PreH27 : (parse_state_6 str_l i level max_level output_l_2 )) ,
+  TT && emp 
+|--
+  “ (parse_state_6 str_l (i + 1 ) (level - 1 ) 0 (app (output_l_2) ((cons (max_level) ((@nil Z))))) ) ” 
+  &&  “ ((out_size + 1 ) = (Zlength ((app (output_l_2) ((cons (max_level) ((@nil Z)))))))) ”
+  &&  emp
+).
+
+Definition parse_nested_parens_entail_wit_3_split_goal_1 := 
+forall (str_l: (@list Z)) (ch: Z) (max_level: Z) (level: Z) (output_l_2: (@list Z)) (out_size: Z) (data: Z) (out: Z) (cap: Z) (n: Z) (i: Z) (PreH1 : (0 <= ((string_length (str_l)) + 1 ))) (PreH2 : ((level - 1 ) = 0)) (PreH3 : ((Znth i (c_string (str_l)) 0) = 41)) (PreH4 : ((Znth i (c_string (str_l)) 0) <> 40)) (PreH5 : (i < n)) (PreH6 : (0 <= i)) (PreH7 : (i <= n)) (PreH8 : (n = (string_length (str_l)))) (PreH9 : (cap = (n + 1 ))) (PreH10 : (out <> 0)) (PreH11 : (data <> 0)) (PreH12 : (0 <= out_size)) (PreH13 : (out_size <= i)) (PreH14 : (out_size = (Zlength (output_l_2)))) (PreH15 : (0 <= level)) (PreH16 : (level <= i)) (PreH17 : (0 <= max_level)) (PreH18 : (max_level <= i)) (PreH19 : (0 <= ch)) (PreH20 : (ch <= 127)) (PreH21 : (valid_string str_l )) (PreH22 : (all_ascii str_l )) (PreH23 : (valid_paren_depth_input_6 str_l )) (PreH24 : (parse_safe_input_6 str_l )) (PreH25 : (((string_length (str_l)) + 1 ) < INT_MAX)) (PreH26 : (problem_6_pre_z str_l )) (PreH27 : (parse_state_6 str_l i level max_level output_l_2 )) ,
+  TT && emp 
+|--
+  “ (parse_state_6 str_l (i + 1 ) (level - 1 ) 0 (app (output_l_2) ((cons (max_level) ((@nil Z))))) ) ”
+.
+
+Definition parse_nested_parens_entail_wit_3_split_goal_2 := 
+forall (str_l: (@list Z)) (ch: Z) (max_level: Z) (level: Z) (output_l_2: (@list Z)) (out_size: Z) (data: Z) (out: Z) (cap: Z) (n: Z) (i: Z) (PreH1 : (0 <= ((string_length (str_l)) + 1 ))) (PreH2 : ((level - 1 ) = 0)) (PreH3 : ((Znth i (c_string (str_l)) 0) = 41)) (PreH4 : ((Znth i (c_string (str_l)) 0) <> 40)) (PreH5 : (i < n)) (PreH6 : (0 <= i)) (PreH7 : (i <= n)) (PreH8 : (n = (string_length (str_l)))) (PreH9 : (cap = (n + 1 ))) (PreH10 : (out <> 0)) (PreH11 : (data <> 0)) (PreH12 : (0 <= out_size)) (PreH13 : (out_size <= i)) (PreH14 : (out_size = (Zlength (output_l_2)))) (PreH15 : (0 <= level)) (PreH16 : (level <= i)) (PreH17 : (0 <= max_level)) (PreH18 : (max_level <= i)) (PreH19 : (0 <= ch)) (PreH20 : (ch <= 127)) (PreH21 : (valid_string str_l )) (PreH22 : (all_ascii str_l )) (PreH23 : (valid_paren_depth_input_6 str_l )) (PreH24 : (parse_safe_input_6 str_l )) (PreH25 : (((string_length (str_l)) + 1 ) < INT_MAX)) (PreH26 : (problem_6_pre_z str_l )) (PreH27 : (parse_state_6 str_l i level max_level output_l_2 )) ,
+  TT && emp 
+|--
+  “ ((out_size + 1 ) = (Zlength ((app (output_l_2) ((cons (max_level) ((@nil Z)))))))) ”
+.
+
+Definition parse_nested_parens_entail_wit_4 := 
+(
+forall (paren_string_pre: Z) (str_l: (@list Z)) (ch: Z) (max_level: Z) (level: Z) (output_l_2: (@list Z)) (out_size: Z) (data: Z) (out: Z) (cap: Z) (n: Z) (i: Z) (PreH1 : ((level - 1 ) <> 0)) (PreH2 : ((Znth i (c_string (str_l)) 0) = 41)) (PreH3 : ((Znth i (c_string (str_l)) 0) <> 40)) (PreH4 : (i < n)) (PreH5 : (0 <= i)) (PreH6 : (i <= n)) (PreH7 : (n = (string_length (str_l)))) (PreH8 : (cap = (n + 1 ))) (PreH9 : (out <> 0)) (PreH10 : (data <> 0)) (PreH11 : (0 <= out_size)) (PreH12 : (out_size <= i)) (PreH13 : (out_size = (Zlength (output_l_2)))) (PreH14 : (0 <= level)) (PreH15 : (level <= i)) (PreH16 : (0 <= max_level)) (PreH17 : (max_level <= i)) (PreH18 : (0 <= ch)) (PreH19 : (ch <= 127)) (PreH20 : (valid_string str_l )) (PreH21 : (all_ascii str_l )) (PreH22 : (valid_paren_depth_input_6 str_l )) (PreH23 : (parse_safe_input_6 str_l )) (PreH24 : (((string_length (str_l)) + 1 ) < INT_MAX)) (PreH25 : (problem_6_pre_z str_l )) (PreH26 : (parse_state_6 str_l i level max_level output_l_2 )) ,
+  (store_string paren_string_pre str_l )
+  **  ((&((out)  # "<anonymous struct>" ->ₛ "data")) # Ptr  |->_)
+  **  ((&((out)  # "<anonymous struct>" ->ₛ "size")) # Int  |->_)
+  **  (IntArray.seg data 0 out_size output_l_2 )
+  **  (IntArray.undef_seg data out_size cap )
+|--
+  EX (output_l: (@list Z)) ,
+  “ (0 <= i) ” 
+  &&  “ (i < n) ” 
+  &&  “ (n = (string_length (str_l))) ” 
+  &&  “ (cap = (n + 1 )) ” 
+  &&  “ (out <> 0) ” 
+  &&  “ (data <> 0) ” 
+  &&  “ ((Znth i (c_string (str_l)) 0) = 41) ” 
+  &&  “ (0 <= out_size) ” 
+  &&  “ (out_size <= i) ” 
+  &&  “ (out_size = (Zlength (output_l))) ” 
+  &&  “ (0 < (level - 1 )) ” 
+  &&  “ ((level - 1 ) <= i) ” 
+  &&  “ (0 <= max_level) ” 
+  &&  “ (max_level <= i) ” 
+  &&  “ (valid_string str_l ) ” 
+  &&  “ (all_ascii str_l ) ” 
+  &&  “ (valid_paren_depth_input_6 str_l ) ” 
+  &&  “ (parse_safe_input_6 str_l ) ” 
+  &&  “ (((string_length (str_l)) + 1 ) < INT_MAX) ” 
+  &&  “ (problem_6_pre_z str_l ) ” 
+  &&  “ (parse_state_6 str_l (i + 1 ) (level - 1 ) max_level output_l ) ”
+  &&  (store_string paren_string_pre str_l )
+  **  ((&((out)  # "<anonymous struct>" ->ₛ "data")) # Ptr  |->_)
+  **  ((&((out)  # "<anonymous struct>" ->ₛ "size")) # Int  |->_)
+  **  (IntArray.seg data 0 out_size output_l )
+  **  (IntArray.undef_seg data out_size cap )
+) \/
+(
+forall (str_l: (@list Z)) (ch: Z) (max_level: Z) (level: Z) (output_l_2: (@list Z)) (out_size: Z) (data: Z) (out: Z) (cap: Z) (n: Z) (i: Z) (PreH1 : (0 <= ((string_length (str_l)) + 1 ))) (PreH2 : ((level - 1 ) <> 0)) (PreH3 : ((Znth i (c_string (str_l)) 0) = 41)) (PreH4 : ((Znth i (c_string (str_l)) 0) <> 40)) (PreH5 : (i < n)) (PreH6 : (0 <= i)) (PreH7 : (i <= n)) (PreH8 : (n = (string_length (str_l)))) (PreH9 : (cap = (n + 1 ))) (PreH10 : (out <> 0)) (PreH11 : (data <> 0)) (PreH12 : (0 <= out_size)) (PreH13 : (out_size <= i)) (PreH14 : (out_size = (Zlength (output_l_2)))) (PreH15 : (0 <= level)) (PreH16 : (level <= i)) (PreH17 : (0 <= max_level)) (PreH18 : (max_level <= i)) (PreH19 : (0 <= ch)) (PreH20 : (ch <= 127)) (PreH21 : (valid_string str_l )) (PreH22 : (all_ascii str_l )) (PreH23 : (valid_paren_depth_input_6 str_l )) (PreH24 : (parse_safe_input_6 str_l )) (PreH25 : (((string_length (str_l)) + 1 ) < INT_MAX)) (PreH26 : (problem_6_pre_z str_l )) (PreH27 : (parse_state_6 str_l i level max_level output_l_2 )) ,
+  TT && emp 
+|--
+  “ (parse_state_6 str_l (i + 1 ) (level - 1 ) max_level output_l_2 ) ” 
+  &&  “ (0 < (level - 1 )) ”
+  &&  emp
+).
+
+Definition parse_nested_parens_entail_wit_4_split_goal_1 := 
+forall (str_l: (@list Z)) (ch: Z) (max_level: Z) (level: Z) (output_l_2: (@list Z)) (out_size: Z) (data: Z) (out: Z) (cap: Z) (n: Z) (i: Z) (PreH1 : (0 <= ((string_length (str_l)) + 1 ))) (PreH2 : ((level - 1 ) <> 0)) (PreH3 : ((Znth i (c_string (str_l)) 0) = 41)) (PreH4 : ((Znth i (c_string (str_l)) 0) <> 40)) (PreH5 : (i < n)) (PreH6 : (0 <= i)) (PreH7 : (i <= n)) (PreH8 : (n = (string_length (str_l)))) (PreH9 : (cap = (n + 1 ))) (PreH10 : (out <> 0)) (PreH11 : (data <> 0)) (PreH12 : (0 <= out_size)) (PreH13 : (out_size <= i)) (PreH14 : (out_size = (Zlength (output_l_2)))) (PreH15 : (0 <= level)) (PreH16 : (level <= i)) (PreH17 : (0 <= max_level)) (PreH18 : (max_level <= i)) (PreH19 : (0 <= ch)) (PreH20 : (ch <= 127)) (PreH21 : (valid_string str_l )) (PreH22 : (all_ascii str_l )) (PreH23 : (valid_paren_depth_input_6 str_l )) (PreH24 : (parse_safe_input_6 str_l )) (PreH25 : (((string_length (str_l)) + 1 ) < INT_MAX)) (PreH26 : (problem_6_pre_z str_l )) (PreH27 : (parse_state_6 str_l i level max_level output_l_2 )) ,
+  TT && emp 
+|--
+  “ (parse_state_6 str_l (i + 1 ) (level - 1 ) max_level output_l_2 ) ”
+.
+
+Definition parse_nested_parens_entail_wit_4_split_goal_2 := 
+forall (str_l: (@list Z)) (ch: Z) (max_level: Z) (level: Z) (output_l_2: (@list Z)) (out_size: Z) (data: Z) (out: Z) (cap: Z) (n: Z) (i: Z) (PreH1 : (0 <= ((string_length (str_l)) + 1 ))) (PreH2 : ((level - 1 ) <> 0)) (PreH3 : ((Znth i (c_string (str_l)) 0) = 41)) (PreH4 : ((Znth i (c_string (str_l)) 0) <> 40)) (PreH5 : (i < n)) (PreH6 : (0 <= i)) (PreH7 : (i <= n)) (PreH8 : (n = (string_length (str_l)))) (PreH9 : (cap = (n + 1 ))) (PreH10 : (out <> 0)) (PreH11 : (data <> 0)) (PreH12 : (0 <= out_size)) (PreH13 : (out_size <= i)) (PreH14 : (out_size = (Zlength (output_l_2)))) (PreH15 : (0 <= level)) (PreH16 : (level <= i)) (PreH17 : (0 <= max_level)) (PreH18 : (max_level <= i)) (PreH19 : (0 <= ch)) (PreH20 : (ch <= 127)) (PreH21 : (valid_string str_l )) (PreH22 : (all_ascii str_l )) (PreH23 : (valid_paren_depth_input_6 str_l )) (PreH24 : (parse_safe_input_6 str_l )) (PreH25 : (((string_length (str_l)) + 1 ) < INT_MAX)) (PreH26 : (problem_6_pre_z str_l )) (PreH27 : (parse_state_6 str_l i level max_level output_l_2 )) ,
+  TT && emp 
+|--
+  “ (0 < (level - 1 )) ”
+.
+
+Definition parse_nested_parens_entail_wit_5 := 
+(
+forall (paren_string_pre: Z) (str_l: (@list Z)) (ch: Z) (max_level: Z) (level: Z) (output_l_2: (@list Z)) (out_size: Z) (data: Z) (out: Z) (cap: Z) (n: Z) (i: Z) (PreH1 : ((Znth i (c_string (str_l)) 0) <> 41)) (PreH2 : ((Znth i (c_string (str_l)) 0) <> 40)) (PreH3 : (i < n)) (PreH4 : (0 <= i)) (PreH5 : (i <= n)) (PreH6 : (n = (string_length (str_l)))) (PreH7 : (cap = (n + 1 ))) (PreH8 : (out <> 0)) (PreH9 : (data <> 0)) (PreH10 : (0 <= out_size)) (PreH11 : (out_size <= i)) (PreH12 : (out_size = (Zlength (output_l_2)))) (PreH13 : (0 <= level)) (PreH14 : (level <= i)) (PreH15 : (0 <= max_level)) (PreH16 : (max_level <= i)) (PreH17 : (0 <= ch)) (PreH18 : (ch <= 127)) (PreH19 : (valid_string str_l )) (PreH20 : (all_ascii str_l )) (PreH21 : (valid_paren_depth_input_6 str_l )) (PreH22 : (parse_safe_input_6 str_l )) (PreH23 : (((string_length (str_l)) + 1 ) < INT_MAX)) (PreH24 : (problem_6_pre_z str_l )) (PreH25 : (parse_state_6 str_l i level max_level output_l_2 )) ,
+  (store_string paren_string_pre str_l )
+  **  ((&((out)  # "<anonymous struct>" ->ₛ "data")) # Ptr  |->_)
+  **  ((&((out)  # "<anonymous struct>" ->ₛ "size")) # Int  |->_)
+  **  (IntArray.seg data 0 out_size output_l_2 )
+  **  (IntArray.undef_seg data out_size cap )
+|--
+  EX (output_l: (@list Z)) ,
+  “ (0 <= i) ” 
+  &&  “ (i < n) ” 
+  &&  “ (n = (string_length (str_l))) ” 
+  &&  “ (cap = (n + 1 )) ” 
+  &&  “ (out <> 0) ” 
+  &&  “ (data <> 0) ” 
+  &&  “ ((Znth i (c_string (str_l)) 0) = 32) ” 
+  &&  “ (0 <= out_size) ” 
+  &&  “ (out_size <= i) ” 
+  &&  “ (out_size = (Zlength (output_l))) ” 
+  &&  “ (0 <= level) ” 
+  &&  “ (level <= i) ” 
+  &&  “ (0 <= max_level) ” 
+  &&  “ (max_level <= i) ” 
+  &&  “ (valid_string str_l ) ” 
+  &&  “ (all_ascii str_l ) ” 
+  &&  “ (valid_paren_depth_input_6 str_l ) ” 
+  &&  “ (parse_safe_input_6 str_l ) ” 
+  &&  “ (((string_length (str_l)) + 1 ) < INT_MAX) ” 
+  &&  “ (problem_6_pre_z str_l ) ” 
+  &&  “ (parse_state_6 str_l (i + 1 ) level max_level output_l ) ”
+  &&  (store_string paren_string_pre str_l )
+  **  ((&((out)  # "<anonymous struct>" ->ₛ "data")) # Ptr  |->_)
+  **  ((&((out)  # "<anonymous struct>" ->ₛ "size")) # Int  |->_)
+  **  (IntArray.seg data 0 out_size output_l )
+  **  (IntArray.undef_seg data out_size cap )
+) \/
+(
+forall (str_l: (@list Z)) (ch: Z) (max_level: Z) (level: Z) (output_l_2: (@list Z)) (out_size: Z) (data: Z) (out: Z) (cap: Z) (n: Z) (i: Z) (PreH1 : (0 <= ((string_length (str_l)) + 1 ))) (PreH2 : ((Znth i (c_string (str_l)) 0) <> 41)) (PreH3 : ((Znth i (c_string (str_l)) 0) <> 40)) (PreH4 : (i < n)) (PreH5 : (0 <= i)) (PreH6 : (i <= n)) (PreH7 : (n = (string_length (str_l)))) (PreH8 : (cap = (n + 1 ))) (PreH9 : (out <> 0)) (PreH10 : (data <> 0)) (PreH11 : (0 <= out_size)) (PreH12 : (out_size <= i)) (PreH13 : (out_size = (Zlength (output_l_2)))) (PreH14 : (0 <= level)) (PreH15 : (level <= i)) (PreH16 : (0 <= max_level)) (PreH17 : (max_level <= i)) (PreH18 : (0 <= ch)) (PreH19 : (ch <= 127)) (PreH20 : (valid_string str_l )) (PreH21 : (all_ascii str_l )) (PreH22 : (valid_paren_depth_input_6 str_l )) (PreH23 : (parse_safe_input_6 str_l )) (PreH24 : (((string_length (str_l)) + 1 ) < INT_MAX)) (PreH25 : (problem_6_pre_z str_l )) (PreH26 : (parse_state_6 str_l i level max_level output_l_2 )) ,
+  TT && emp 
+|--
+  “ (parse_state_6 str_l (i + 1 ) level max_level output_l_2 ) ” 
+  &&  “ ((Znth i (c_string (str_l)) 0) = 32) ”
+  &&  emp
+).
+
+Definition parse_nested_parens_entail_wit_5_split_goal_1 := 
+forall (str_l: (@list Z)) (ch: Z) (max_level: Z) (level: Z) (output_l_2: (@list Z)) (out_size: Z) (data: Z) (out: Z) (cap: Z) (n: Z) (i: Z) (PreH1 : (0 <= ((string_length (str_l)) + 1 ))) (PreH2 : ((Znth i (c_string (str_l)) 0) <> 41)) (PreH3 : ((Znth i (c_string (str_l)) 0) <> 40)) (PreH4 : (i < n)) (PreH5 : (0 <= i)) (PreH6 : (i <= n)) (PreH7 : (n = (string_length (str_l)))) (PreH8 : (cap = (n + 1 ))) (PreH9 : (out <> 0)) (PreH10 : (data <> 0)) (PreH11 : (0 <= out_size)) (PreH12 : (out_size <= i)) (PreH13 : (out_size = (Zlength (output_l_2)))) (PreH14 : (0 <= level)) (PreH15 : (level <= i)) (PreH16 : (0 <= max_level)) (PreH17 : (max_level <= i)) (PreH18 : (0 <= ch)) (PreH19 : (ch <= 127)) (PreH20 : (valid_string str_l )) (PreH21 : (all_ascii str_l )) (PreH22 : (valid_paren_depth_input_6 str_l )) (PreH23 : (parse_safe_input_6 str_l )) (PreH24 : (((string_length (str_l)) + 1 ) < INT_MAX)) (PreH25 : (problem_6_pre_z str_l )) (PreH26 : (parse_state_6 str_l i level max_level output_l_2 )) ,
+  TT && emp 
+|--
+  “ (parse_state_6 str_l (i + 1 ) level max_level output_l_2 ) ”
+.
+
+Definition parse_nested_parens_entail_wit_5_split_goal_2 := 
+forall (str_l: (@list Z)) (ch: Z) (max_level: Z) (level: Z) (output_l_2: (@list Z)) (out_size: Z) (data: Z) (out: Z) (cap: Z) (n: Z) (i: Z) (PreH1 : (0 <= ((string_length (str_l)) + 1 ))) (PreH2 : ((Znth i (c_string (str_l)) 0) <> 41)) (PreH3 : ((Znth i (c_string (str_l)) 0) <> 40)) (PreH4 : (i < n)) (PreH5 : (0 <= i)) (PreH6 : (i <= n)) (PreH7 : (n = (string_length (str_l)))) (PreH8 : (cap = (n + 1 ))) (PreH9 : (out <> 0)) (PreH10 : (data <> 0)) (PreH11 : (0 <= out_size)) (PreH12 : (out_size <= i)) (PreH13 : (out_size = (Zlength (output_l_2)))) (PreH14 : (0 <= level)) (PreH15 : (level <= i)) (PreH16 : (0 <= max_level)) (PreH17 : (max_level <= i)) (PreH18 : (0 <= ch)) (PreH19 : (ch <= 127)) (PreH20 : (valid_string str_l )) (PreH21 : (all_ascii str_l )) (PreH22 : (valid_paren_depth_input_6 str_l )) (PreH23 : (parse_safe_input_6 str_l )) (PreH24 : (((string_length (str_l)) + 1 ) < INT_MAX)) (PreH25 : (problem_6_pre_z str_l )) (PreH26 : (parse_state_6 str_l i level max_level output_l_2 )) ,
+  TT && emp 
+|--
+  “ ((Znth i (c_string (str_l)) 0) = 32) ”
+.
+
+Definition parse_nested_parens_entail_wit_6_1 := 
+forall (paren_string_pre: Z) (str_l: (@list Z)) (output_l_2: (@list Z)) (i: Z) (n: Z) (cap: Z) (out: Z) (data: Z) (ch: Z) (out_size: Z) (level: Z) (max_level: Z) (PreH1 : (0 <= i)) (PreH2 : (i < n)) (PreH3 : (n = (string_length (str_l)))) (PreH4 : (cap = (n + 1 ))) (PreH5 : (out <> 0)) (PreH6 : (data <> 0)) (PreH7 : (ch = 40)) (PreH8 : (0 <= out_size)) (PreH9 : (out_size <= i)) (PreH10 : (out_size = (Zlength (output_l_2)))) (PreH11 : (1 <= level)) (PreH12 : (level <= (i + 1 ))) (PreH13 : (1 <= max_level)) (PreH14 : (max_level <= (i + 1 ))) (PreH15 : (valid_string str_l )) (PreH16 : (all_ascii str_l )) (PreH17 : (valid_paren_depth_input_6 str_l )) (PreH18 : (parse_safe_input_6 str_l )) (PreH19 : (((string_length (str_l)) + 1 ) < INT_MAX)) (PreH20 : (problem_6_pre_z str_l )) (PreH21 : (parse_state_6 str_l (i + 1 ) level max_level output_l_2 )) ,
+  (store_string paren_string_pre str_l )
+  **  ((&((out)  # "<anonymous struct>" ->ₛ "data")) # Ptr  |->_)
+  **  ((&((out)  # "<anonymous struct>" ->ₛ "size")) # Int  |->_)
+  **  (IntArray.seg data 0 out_size output_l_2 )
+  **  (IntArray.undef_seg data out_size cap )
+|--
+  EX (output_l: (@list Z)) ,
+  “ (0 <= (i + 1 )) ” 
+  &&  “ ((i + 1 ) <= n) ” 
+  &&  “ (n = (string_length (str_l))) ” 
+  &&  “ (cap = (n + 1 )) ” 
+  &&  “ (out <> 0) ” 
+  &&  “ (data <> 0) ” 
+  &&  “ (0 <= out_size) ” 
+  &&  “ (out_size <= (i + 1 )) ” 
+  &&  “ (out_size = (Zlength (output_l))) ” 
+  &&  “ (0 <= level) ” 
+  &&  “ (level <= (i + 1 )) ” 
+  &&  “ (0 <= max_level) ” 
+  &&  “ (max_level <= (i + 1 )) ” 
+  &&  “ (0 <= ch) ” 
+  &&  “ (ch <= 127) ” 
+  &&  “ (valid_string str_l ) ” 
+  &&  “ (all_ascii str_l ) ” 
+  &&  “ (valid_paren_depth_input_6 str_l ) ” 
+  &&  “ (parse_safe_input_6 str_l ) ” 
+  &&  “ (((string_length (str_l)) + 1 ) < INT_MAX) ” 
+  &&  “ (problem_6_pre_z str_l ) ” 
+  &&  “ (parse_state_6 str_l (i + 1 ) level max_level output_l ) ”
+  &&  (store_string paren_string_pre str_l )
+  **  ((&((out)  # "<anonymous struct>" ->ₛ "data")) # Ptr  |->_)
+  **  ((&((out)  # "<anonymous struct>" ->ₛ "size")) # Int  |->_)
+  **  (IntArray.seg data 0 out_size output_l )
+  **  (IntArray.undef_seg data out_size cap )
+.
+
+Definition parse_nested_parens_entail_wit_6_2 := 
+forall (paren_string_pre: Z) (str_l: (@list Z)) (output_l_2: (@list Z)) (i: Z) (n: Z) (cap: Z) (out: Z) (data: Z) (ch: Z) (out_size: Z) (level: Z) (max_level: Z) (PreH1 : (0 <= i)) (PreH2 : (i < n)) (PreH3 : (n = (string_length (str_l)))) (PreH4 : (cap = (n + 1 ))) (PreH5 : (out <> 0)) (PreH6 : (data <> 0)) (PreH7 : (ch = 41)) (PreH8 : (1 <= out_size)) (PreH9 : (out_size <= (i + 1 ))) (PreH10 : (out_size = (Zlength (output_l_2)))) (PreH11 : (level = 0)) (PreH12 : (max_level = 0)) (PreH13 : (valid_string str_l )) (PreH14 : (all_ascii str_l )) (PreH15 : (valid_paren_depth_input_6 str_l )) (PreH16 : (parse_safe_input_6 str_l )) (PreH17 : (((string_length (str_l)) + 1 ) < INT_MAX)) (PreH18 : (problem_6_pre_z str_l )) (PreH19 : (parse_state_6 str_l (i + 1 ) level max_level output_l_2 )) ,
+  (store_string paren_string_pre str_l )
+  **  ((&((out)  # "<anonymous struct>" ->ₛ "data")) # Ptr  |->_)
+  **  ((&((out)  # "<anonymous struct>" ->ₛ "size")) # Int  |->_)
+  **  (IntArray.seg data 0 out_size output_l_2 )
+  **  (IntArray.undef_seg data out_size cap )
+|--
+  EX (output_l: (@list Z)) ,
+  “ (0 <= (i + 1 )) ” 
+  &&  “ ((i + 1 ) <= n) ” 
+  &&  “ (n = (string_length (str_l))) ” 
+  &&  “ (cap = (n + 1 )) ” 
+  &&  “ (out <> 0) ” 
+  &&  “ (data <> 0) ” 
+  &&  “ (0 <= out_size) ” 
+  &&  “ (out_size <= (i + 1 )) ” 
+  &&  “ (out_size = (Zlength (output_l))) ” 
+  &&  “ (0 <= level) ” 
+  &&  “ (level <= (i + 1 )) ” 
+  &&  “ (0 <= max_level) ” 
+  &&  “ (max_level <= (i + 1 )) ” 
+  &&  “ (0 <= ch) ” 
+  &&  “ (ch <= 127) ” 
+  &&  “ (valid_string str_l ) ” 
+  &&  “ (all_ascii str_l ) ” 
+  &&  “ (valid_paren_depth_input_6 str_l ) ” 
+  &&  “ (parse_safe_input_6 str_l ) ” 
+  &&  “ (((string_length (str_l)) + 1 ) < INT_MAX) ” 
+  &&  “ (problem_6_pre_z str_l ) ” 
+  &&  “ (parse_state_6 str_l (i + 1 ) level max_level output_l ) ”
+  &&  (store_string paren_string_pre str_l )
+  **  ((&((out)  # "<anonymous struct>" ->ₛ "data")) # Ptr  |->_)
+  **  ((&((out)  # "<anonymous struct>" ->ₛ "size")) # Int  |->_)
+  **  (IntArray.seg data 0 out_size output_l )
+  **  (IntArray.undef_seg data out_size cap )
+.
+
+Definition parse_nested_parens_entail_wit_6_3 := 
+forall (paren_string_pre: Z) (str_l: (@list Z)) (output_l_2: (@list Z)) (i: Z) (n: Z) (cap: Z) (out: Z) (data: Z) (ch: Z) (out_size: Z) (level: Z) (max_level: Z) (PreH1 : (0 <= i)) (PreH2 : (i < n)) (PreH3 : (n = (string_length (str_l)))) (PreH4 : (cap = (n + 1 ))) (PreH5 : (out <> 0)) (PreH6 : (data <> 0)) (PreH7 : (ch = 41)) (PreH8 : (0 <= out_size)) (PreH9 : (out_size <= i)) (PreH10 : (out_size = (Zlength (output_l_2)))) (PreH11 : (0 < level)) (PreH12 : (level <= i)) (PreH13 : (0 <= max_level)) (PreH14 : (max_level <= i)) (PreH15 : (valid_string str_l )) (PreH16 : (all_ascii str_l )) (PreH17 : (valid_paren_depth_input_6 str_l )) (PreH18 : (parse_safe_input_6 str_l )) (PreH19 : (((string_length (str_l)) + 1 ) < INT_MAX)) (PreH20 : (problem_6_pre_z str_l )) (PreH21 : (parse_state_6 str_l (i + 1 ) level max_level output_l_2 )) ,
+  (store_string paren_string_pre str_l )
+  **  ((&((out)  # "<anonymous struct>" ->ₛ "data")) # Ptr  |->_)
+  **  ((&((out)  # "<anonymous struct>" ->ₛ "size")) # Int  |->_)
+  **  (IntArray.seg data 0 out_size output_l_2 )
+  **  (IntArray.undef_seg data out_size cap )
+|--
+  EX (output_l: (@list Z)) ,
+  “ (0 <= (i + 1 )) ” 
+  &&  “ ((i + 1 ) <= n) ” 
+  &&  “ (n = (string_length (str_l))) ” 
+  &&  “ (cap = (n + 1 )) ” 
+  &&  “ (out <> 0) ” 
+  &&  “ (data <> 0) ” 
+  &&  “ (0 <= out_size) ” 
+  &&  “ (out_size <= (i + 1 )) ” 
+  &&  “ (out_size = (Zlength (output_l))) ” 
+  &&  “ (0 <= level) ” 
+  &&  “ (level <= (i + 1 )) ” 
+  &&  “ (0 <= max_level) ” 
+  &&  “ (max_level <= (i + 1 )) ” 
+  &&  “ (0 <= ch) ” 
+  &&  “ (ch <= 127) ” 
+  &&  “ (valid_string str_l ) ” 
+  &&  “ (all_ascii str_l ) ” 
+  &&  “ (valid_paren_depth_input_6 str_l ) ” 
+  &&  “ (parse_safe_input_6 str_l ) ” 
+  &&  “ (((string_length (str_l)) + 1 ) < INT_MAX) ” 
+  &&  “ (problem_6_pre_z str_l ) ” 
+  &&  “ (parse_state_6 str_l (i + 1 ) level max_level output_l ) ”
+  &&  (store_string paren_string_pre str_l )
+  **  ((&((out)  # "<anonymous struct>" ->ₛ "data")) # Ptr  |->_)
+  **  ((&((out)  # "<anonymous struct>" ->ₛ "size")) # Int  |->_)
+  **  (IntArray.seg data 0 out_size output_l )
+  **  (IntArray.undef_seg data out_size cap )
+.
+
+Definition parse_nested_parens_entail_wit_6_4 := 
+forall (paren_string_pre: Z) (str_l: (@list Z)) (output_l_2: (@list Z)) (i: Z) (n: Z) (cap: Z) (out: Z) (data: Z) (ch: Z) (out_size: Z) (level: Z) (max_level: Z) (PreH1 : (0 <= i)) (PreH2 : (i < n)) (PreH3 : (n = (string_length (str_l)))) (PreH4 : (cap = (n + 1 ))) (PreH5 : (out <> 0)) (PreH6 : (data <> 0)) (PreH7 : (ch = 32)) (PreH8 : (0 <= out_size)) (PreH9 : (out_size <= i)) (PreH10 : (out_size = (Zlength (output_l_2)))) (PreH11 : (0 <= level)) (PreH12 : (level <= i)) (PreH13 : (0 <= max_level)) (PreH14 : (max_level <= i)) (PreH15 : (valid_string str_l )) (PreH16 : (all_ascii str_l )) (PreH17 : (valid_paren_depth_input_6 str_l )) (PreH18 : (parse_safe_input_6 str_l )) (PreH19 : (((string_length (str_l)) + 1 ) < INT_MAX)) (PreH20 : (problem_6_pre_z str_l )) (PreH21 : (parse_state_6 str_l (i + 1 ) level max_level output_l_2 )) ,
+  (store_string paren_string_pre str_l )
+  **  ((&((out)  # "<anonymous struct>" ->ₛ "data")) # Ptr  |->_)
+  **  ((&((out)  # "<anonymous struct>" ->ₛ "size")) # Int  |->_)
+  **  (IntArray.seg data 0 out_size output_l_2 )
+  **  (IntArray.undef_seg data out_size cap )
+|--
+  EX (output_l: (@list Z)) ,
+  “ (0 <= (i + 1 )) ” 
+  &&  “ ((i + 1 ) <= n) ” 
+  &&  “ (n = (string_length (str_l))) ” 
+  &&  “ (cap = (n + 1 )) ” 
+  &&  “ (out <> 0) ” 
+  &&  “ (data <> 0) ” 
+  &&  “ (0 <= out_size) ” 
+  &&  “ (out_size <= (i + 1 )) ” 
+  &&  “ (out_size = (Zlength (output_l))) ” 
+  &&  “ (0 <= level) ” 
+  &&  “ (level <= (i + 1 )) ” 
+  &&  “ (0 <= max_level) ” 
+  &&  “ (max_level <= (i + 1 )) ” 
+  &&  “ (0 <= ch) ” 
+  &&  “ (ch <= 127) ” 
+  &&  “ (valid_string str_l ) ” 
+  &&  “ (all_ascii str_l ) ” 
+  &&  “ (valid_paren_depth_input_6 str_l ) ” 
+  &&  “ (parse_safe_input_6 str_l ) ” 
+  &&  “ (((string_length (str_l)) + 1 ) < INT_MAX) ” 
+  &&  “ (problem_6_pre_z str_l ) ” 
+  &&  “ (parse_state_6 str_l (i + 1 ) level max_level output_l ) ”
+  &&  (store_string paren_string_pre str_l )
+  **  ((&((out)  # "<anonymous struct>" ->ₛ "data")) # Ptr  |->_)
+  **  ((&((out)  # "<anonymous struct>" ->ₛ "size")) # Int  |->_)
+  **  (IntArray.seg data 0 out_size output_l )
+  **  (IntArray.undef_seg data out_size cap )
+.
+
+Definition parse_nested_parens_entail_wit_7 := 
+(
+forall (paren_string_pre: Z) (str_l: (@list Z)) (ch: Z) (max_level: Z) (level: Z) (output_l_2: (@list Z)) (out_size: Z) (data: Z) (out: Z) (cap: Z) (n: Z) (i: Z) (PreH1 : (i >= n)) (PreH2 : (0 <= i)) (PreH3 : (i <= n)) (PreH4 : (n = (string_length (str_l)))) (PreH5 : (cap = (n + 1 ))) (PreH6 : (out <> 0)) (PreH7 : (data <> 0)) (PreH8 : (0 <= out_size)) (PreH9 : (out_size <= i)) (PreH10 : (out_size = (Zlength (output_l_2)))) (PreH11 : (0 <= level)) (PreH12 : (level <= i)) (PreH13 : (0 <= max_level)) (PreH14 : (max_level <= i)) (PreH15 : (0 <= ch)) (PreH16 : (ch <= 127)) (PreH17 : (valid_string str_l )) (PreH18 : (all_ascii str_l )) (PreH19 : (valid_paren_depth_input_6 str_l )) (PreH20 : (parse_safe_input_6 str_l )) (PreH21 : (((string_length (str_l)) + 1 ) < INT_MAX)) (PreH22 : (problem_6_pre_z str_l )) (PreH23 : (parse_state_6 str_l i level max_level output_l_2 )) ,
+  (store_string paren_string_pre str_l )
+  **  ((&((out)  # "<anonymous struct>" ->ₛ "data")) # Ptr  |->_)
+  **  ((&((out)  # "<anonymous struct>" ->ₛ "size")) # Int  |->_)
+  **  (IntArray.seg data 0 out_size output_l_2 )
+  **  (IntArray.undef_seg data out_size cap )
+|--
+  EX (output_l: (@list Z)) ,
+  “ (n = (string_length (str_l))) ” 
+  &&  “ (cap = (n + 1 )) ” 
+  &&  “ (out <> 0) ” 
+  &&  “ (data <> 0) ” 
+  &&  “ (out_size = (Zlength (output_l))) ” 
+  &&  “ (out_size <= n) ” 
+  &&  “ (level = 0) ” 
+  &&  “ (max_level = 0) ” 
+  &&  “ (output_l = (parse_output_6 (str_l))) ” 
+  &&  “ (valid_string str_l ) ” 
+  &&  “ (all_ascii str_l ) ” 
+  &&  “ (valid_paren_depth_input_6 str_l ) ” 
+  &&  “ (parse_safe_input_6 str_l ) ” 
+  &&  “ (((string_length (str_l)) + 1 ) < INT_MAX) ” 
+  &&  “ (problem_6_pre_z str_l ) ” 
+  &&  “ (problem_6_spec_z str_l output_l ) ”
+  &&  (store_string paren_string_pre str_l )
+  **  ((&((out)  # "<anonymous struct>" ->ₛ "data")) # Ptr  |->_)
+  **  ((&((out)  # "<anonymous struct>" ->ₛ "size")) # Int  |->_)
+  **  (IntArray.seg data 0 out_size output_l )
+  **  (IntArray.undef_seg data out_size cap )
+) \/
+(
+forall (str_l: (@list Z)) (ch: Z) (max_level: Z) (level: Z) (output_l_2: (@list Z)) (out_size: Z) (data: Z) (out: Z) (cap: Z) (n: Z) (i: Z) (PreH1 : (0 <= ((string_length (str_l)) + 1 ))) (PreH2 : (i >= n)) (PreH3 : (0 <= i)) (PreH4 : (i <= n)) (PreH5 : (n = (string_length (str_l)))) (PreH6 : (cap = (n + 1 ))) (PreH7 : (out <> 0)) (PreH8 : (data <> 0)) (PreH9 : (0 <= out_size)) (PreH10 : (out_size <= i)) (PreH11 : (out_size = (Zlength (output_l_2)))) (PreH12 : (0 <= level)) (PreH13 : (level <= i)) (PreH14 : (0 <= max_level)) (PreH15 : (max_level <= i)) (PreH16 : (0 <= ch)) (PreH17 : (ch <= 127)) (PreH18 : (valid_string str_l )) (PreH19 : (all_ascii str_l )) (PreH20 : (valid_paren_depth_input_6 str_l )) (PreH21 : (parse_safe_input_6 str_l )) (PreH22 : (((string_length (str_l)) + 1 ) < INT_MAX)) (PreH23 : (problem_6_pre_z str_l )) (PreH24 : (parse_state_6 str_l i level max_level output_l_2 )) ,
+  TT && emp 
+|--
+  “ (problem_6_spec_z str_l (parse_output_6 (str_l)) ) ” 
+  &&  “ (max_level = 0) ” 
+  &&  “ (level = 0) ” 
+  &&  “ (out_size = (Zlength ((parse_output_6 (str_l))))) ” 
+  &&  “ (output_l_2 = (parse_output_6 (str_l))) ”
+  &&  emp
+).
+
+Definition parse_nested_parens_entail_wit_7_split_goal_1 := 
+forall (str_l: (@list Z)) (ch: Z) (max_level: Z) (level: Z) (output_l_2: (@list Z)) (out_size: Z) (data: Z) (out: Z) (cap: Z) (n: Z) (i: Z) (PreH1 : (0 <= ((string_length (str_l)) + 1 ))) (PreH2 : (i >= n)) (PreH3 : (0 <= i)) (PreH4 : (i <= n)) (PreH5 : (n = (string_length (str_l)))) (PreH6 : (cap = (n + 1 ))) (PreH7 : (out <> 0)) (PreH8 : (data <> 0)) (PreH9 : (0 <= out_size)) (PreH10 : (out_size <= i)) (PreH11 : (out_size = (Zlength (output_l_2)))) (PreH12 : (0 <= level)) (PreH13 : (level <= i)) (PreH14 : (0 <= max_level)) (PreH15 : (max_level <= i)) (PreH16 : (0 <= ch)) (PreH17 : (ch <= 127)) (PreH18 : (valid_string str_l )) (PreH19 : (all_ascii str_l )) (PreH20 : (valid_paren_depth_input_6 str_l )) (PreH21 : (parse_safe_input_6 str_l )) (PreH22 : (((string_length (str_l)) + 1 ) < INT_MAX)) (PreH23 : (problem_6_pre_z str_l )) (PreH24 : (parse_state_6 str_l i level max_level output_l_2 )) ,
+  TT && emp 
+|--
+  “ (problem_6_spec_z str_l (parse_output_6 (str_l)) ) ”
+.
+
+Definition parse_nested_parens_entail_wit_7_split_goal_2 := 
+forall (str_l: (@list Z)) (ch: Z) (max_level: Z) (level: Z) (output_l_2: (@list Z)) (out_size: Z) (data: Z) (out: Z) (cap: Z) (n: Z) (i: Z) (PreH1 : (0 <= ((string_length (str_l)) + 1 ))) (PreH2 : (i >= n)) (PreH3 : (0 <= i)) (PreH4 : (i <= n)) (PreH5 : (n = (string_length (str_l)))) (PreH6 : (cap = (n + 1 ))) (PreH7 : (out <> 0)) (PreH8 : (data <> 0)) (PreH9 : (0 <= out_size)) (PreH10 : (out_size <= i)) (PreH11 : (out_size = (Zlength (output_l_2)))) (PreH12 : (0 <= level)) (PreH13 : (level <= i)) (PreH14 : (0 <= max_level)) (PreH15 : (max_level <= i)) (PreH16 : (0 <= ch)) (PreH17 : (ch <= 127)) (PreH18 : (valid_string str_l )) (PreH19 : (all_ascii str_l )) (PreH20 : (valid_paren_depth_input_6 str_l )) (PreH21 : (parse_safe_input_6 str_l )) (PreH22 : (((string_length (str_l)) + 1 ) < INT_MAX)) (PreH23 : (problem_6_pre_z str_l )) (PreH24 : (parse_state_6 str_l i level max_level output_l_2 )) ,
+  TT && emp 
+|--
+  “ (max_level = 0) ”
+.
+
+Definition parse_nested_parens_entail_wit_7_split_goal_3 := 
+forall (str_l: (@list Z)) (ch: Z) (max_level: Z) (level: Z) (output_l_2: (@list Z)) (out_size: Z) (data: Z) (out: Z) (cap: Z) (n: Z) (i: Z) (PreH1 : (0 <= ((string_length (str_l)) + 1 ))) (PreH2 : (i >= n)) (PreH3 : (0 <= i)) (PreH4 : (i <= n)) (PreH5 : (n = (string_length (str_l)))) (PreH6 : (cap = (n + 1 ))) (PreH7 : (out <> 0)) (PreH8 : (data <> 0)) (PreH9 : (0 <= out_size)) (PreH10 : (out_size <= i)) (PreH11 : (out_size = (Zlength (output_l_2)))) (PreH12 : (0 <= level)) (PreH13 : (level <= i)) (PreH14 : (0 <= max_level)) (PreH15 : (max_level <= i)) (PreH16 : (0 <= ch)) (PreH17 : (ch <= 127)) (PreH18 : (valid_string str_l )) (PreH19 : (all_ascii str_l )) (PreH20 : (valid_paren_depth_input_6 str_l )) (PreH21 : (parse_safe_input_6 str_l )) (PreH22 : (((string_length (str_l)) + 1 ) < INT_MAX)) (PreH23 : (problem_6_pre_z str_l )) (PreH24 : (parse_state_6 str_l i level max_level output_l_2 )) ,
+  TT && emp 
+|--
+  “ (level = 0) ”
+.
+
+Definition parse_nested_parens_entail_wit_7_split_goal_4 := 
+forall (str_l: (@list Z)) (ch: Z) (max_level: Z) (level: Z) (output_l_2: (@list Z)) (out_size: Z) (data: Z) (out: Z) (cap: Z) (n: Z) (i: Z) (PreH1 : (0 <= ((string_length (str_l)) + 1 ))) (PreH2 : (i >= n)) (PreH3 : (0 <= i)) (PreH4 : (i <= n)) (PreH5 : (n = (string_length (str_l)))) (PreH6 : (cap = (n + 1 ))) (PreH7 : (out <> 0)) (PreH8 : (data <> 0)) (PreH9 : (0 <= out_size)) (PreH10 : (out_size <= i)) (PreH11 : (out_size = (Zlength (output_l_2)))) (PreH12 : (0 <= level)) (PreH13 : (level <= i)) (PreH14 : (0 <= max_level)) (PreH15 : (max_level <= i)) (PreH16 : (0 <= ch)) (PreH17 : (ch <= 127)) (PreH18 : (valid_string str_l )) (PreH19 : (all_ascii str_l )) (PreH20 : (valid_paren_depth_input_6 str_l )) (PreH21 : (parse_safe_input_6 str_l )) (PreH22 : (((string_length (str_l)) + 1 ) < INT_MAX)) (PreH23 : (problem_6_pre_z str_l )) (PreH24 : (parse_state_6 str_l i level max_level output_l_2 )) ,
+  TT && emp 
+|--
+  “ (out_size = (Zlength ((parse_output_6 (str_l))))) ”
+.
+
+Definition parse_nested_parens_entail_wit_7_split_goal_5 := 
+forall (str_l: (@list Z)) (ch: Z) (max_level: Z) (level: Z) (output_l_2: (@list Z)) (out_size: Z) (data: Z) (out: Z) (cap: Z) (n: Z) (i: Z) (PreH1 : (0 <= ((string_length (str_l)) + 1 ))) (PreH2 : (i >= n)) (PreH3 : (0 <= i)) (PreH4 : (i <= n)) (PreH5 : (n = (string_length (str_l)))) (PreH6 : (cap = (n + 1 ))) (PreH7 : (out <> 0)) (PreH8 : (data <> 0)) (PreH9 : (0 <= out_size)) (PreH10 : (out_size <= i)) (PreH11 : (out_size = (Zlength (output_l_2)))) (PreH12 : (0 <= level)) (PreH13 : (level <= i)) (PreH14 : (0 <= max_level)) (PreH15 : (max_level <= i)) (PreH16 : (0 <= ch)) (PreH17 : (ch <= 127)) (PreH18 : (valid_string str_l )) (PreH19 : (all_ascii str_l )) (PreH20 : (valid_paren_depth_input_6 str_l )) (PreH21 : (parse_safe_input_6 str_l )) (PreH22 : (((string_length (str_l)) + 1 ) < INT_MAX)) (PreH23 : (problem_6_pre_z str_l )) (PreH24 : (parse_state_6 str_l i level max_level output_l_2 )) ,
+  TT && emp 
+|--
+  “ (output_l_2 = (parse_output_6 (str_l))) ”
+.
+
+Definition parse_nested_parens_entail_wit_8 := 
+forall (paren_string_pre: Z) (str_l: (@list Z)) (output_l_2: (@list Z)) (n: Z) (cap: Z) (out: Z) (data: Z) (out_size: Z) (level: Z) (max_level: Z) (PreH1 : (n = (string_length (str_l)))) (PreH2 : (cap = (n + 1 ))) (PreH3 : (out <> 0)) (PreH4 : (data <> 0)) (PreH5 : (out_size = (Zlength (output_l_2)))) (PreH6 : (out_size <= n)) (PreH7 : (level = 0)) (PreH8 : (max_level = 0)) (PreH9 : (output_l_2 = (parse_output_6 (str_l)))) (PreH10 : (valid_string str_l )) (PreH11 : (all_ascii str_l )) (PreH12 : (valid_paren_depth_input_6 str_l )) (PreH13 : (parse_safe_input_6 str_l )) (PreH14 : (((string_length (str_l)) + 1 ) < INT_MAX)) (PreH15 : (problem_6_pre_z str_l )) (PreH16 : (problem_6_spec_z str_l output_l_2 )) ,
+  (store_string paren_string_pre str_l )
+  **  ((&((out)  # "<anonymous struct>" ->ₛ "data")) # Ptr  |-> data)
+  **  ((&((out)  # "<anonymous struct>" ->ₛ "size")) # Int  |-> out_size)
+  **  (IntArray.seg data 0 out_size output_l_2 )
+  **  (IntArray.undef_seg data out_size cap )
+|--
+  EX (output_l: (@list Z)) ,
+  “ (n = (string_length (str_l))) ” 
+  &&  “ (cap = (n + 1 )) ” 
+  &&  “ (out <> 0) ” 
+  &&  “ (data <> 0) ” 
+  &&  “ (out_size = (Zlength (output_l))) ” 
+  &&  “ (out_size <= n) ” 
+  &&  “ (level = 0) ” 
+  &&  “ (max_level = 0) ” 
+  &&  “ (output_l = (parse_output_6 (str_l))) ” 
+  &&  “ (problem_6_spec_z str_l output_l ) ”
+  &&  (store_string paren_string_pre str_l )
+  **  ((&((out)  # "<anonymous struct>" ->ₛ "data")) # Ptr  |-> data)
+  **  ((&((out)  # "<anonymous struct>" ->ₛ "size")) # Int  |-> out_size)
+  **  (IntArray.seg data 0 out_size output_l )
+  **  (IntArray.undef_seg data out_size cap )
+.
+
+Definition parse_nested_parens_return_wit_1 := 
+(
+forall (paren_string_pre: Z) (str_l: (@list Z)) (output_l_2: (@list Z)) (n: Z) (cap: Z) (out: Z) (data_2: Z) (out_size: Z) (level: Z) (max_level: Z) (PreH1 : (n = (string_length (str_l)))) (PreH2 : (cap = (n + 1 ))) (PreH3 : (out <> 0)) (PreH4 : (data_2 <> 0)) (PreH5 : (out_size = (Zlength (output_l_2)))) (PreH6 : (out_size <= n)) (PreH7 : (level = 0)) (PreH8 : (max_level = 0)) (PreH9 : (output_l_2 = (parse_output_6 (str_l)))) (PreH10 : (problem_6_spec_z str_l output_l_2 )) ,
+  (store_string paren_string_pre str_l )
+  **  ((&((out)  # "<anonymous struct>" ->ₛ "data")) # Ptr  |-> data_2)
+  **  ((&((out)  # "<anonymous struct>" ->ₛ "size")) # Int  |-> out_size)
+  **  (IntArray.seg data_2 0 out_size output_l_2 )
+  **  (IntArray.undef_seg data_2 out_size cap )
+|--
+  EX (output_l: (@list Z))  (data: Z) ,
+  “ (out <> 0) ” 
+  &&  “ (data <> 0) ” 
+  &&  “ (output_l = (parse_output_6 (str_l))) ” 
+  &&  “ ((Zlength (output_l)) <= (string_length (str_l))) ” 
+  &&  “ (problem_6_spec_z str_l output_l ) ”
+  &&  (store_string paren_string_pre str_l )
+  **  ((&((out)  # "<anonymous struct>" ->ₛ "data")) # Ptr  |-> data)
+  **  ((&((out)  # "<anonymous struct>" ->ₛ "size")) # Int  |-> (Zlength (output_l)))
+  **  (IntArray.seg data 0 (Zlength (output_l)) output_l )
+  **  (IntArray.undef_seg data (Zlength (output_l)) ((string_length (str_l)) + 1 ) )
+) \/
+(
+forall (str_l: (@list Z)) (output_l_2: (@list Z)) (n: Z) (cap: Z) (out: Z) (data_2: Z) (out_size: Z) (level: Z) (max_level: Z) (PreH1 : (0 <= ((string_length (str_l)) + 1 ))) (PreH2 : (n = (string_length (str_l)))) (PreH3 : (cap = (n + 1 ))) (PreH4 : (out <> 0)) (PreH5 : (data_2 <> 0)) (PreH6 : (out_size = (Zlength (output_l_2)))) (PreH7 : (out_size <= n)) (PreH8 : (level = 0)) (PreH9 : (max_level = 0)) (PreH10 : (output_l_2 = (parse_output_6 (str_l)))) (PreH11 : (problem_6_spec_z str_l output_l_2 )) ,
+  (IntArray.seg data_2 0 out_size output_l_2 )
+|--
+  (IntArray.seg data_2 0 (Zlength ((parse_output_6 (str_l)))) (parse_output_6 (str_l)) )
+).
+
+Definition parse_nested_parens_return_wit_1_split_goal_spatial := 
+forall (str_l: (@list Z)) (output_l_2: (@list Z)) (n: Z) (cap: Z) (out: Z) (data_2: Z) (out_size: Z) (level: Z) (max_level: Z) (PreH1 : (0 <= ((string_length (str_l)) + 1 ))) (PreH2 : (n = (string_length (str_l)))) (PreH3 : (cap = (n + 1 ))) (PreH4 : (out <> 0)) (PreH5 : (data_2 <> 0)) (PreH6 : (out_size = (Zlength (output_l_2)))) (PreH7 : (out_size <= n)) (PreH8 : (level = 0)) (PreH9 : (max_level = 0)) (PreH10 : (output_l_2 = (parse_output_6 (str_l)))) (PreH11 : (problem_6_spec_z str_l output_l_2 )) ,
+  (IntArray.seg data_2 0 out_size output_l_2 )
+|--
+  (IntArray.seg data_2 0 (Zlength ((parse_output_6 (str_l)))) (parse_output_6 (str_l)) )
+.
+
+Definition parse_nested_parens_partial_solve_wit_1_pure := 
+forall (paren_string_pre: Z) (str_l: (@list Z)) (PreH1 : (valid_string str_l )) (PreH2 : (all_ascii str_l )) (PreH3 : (valid_paren_depth_input_6 str_l )) (PreH4 : (parse_safe_input_6 str_l )) (PreH5 : (((string_length (str_l)) + 1 ) < INT_MAX)) (PreH6 : (problem_6_pre_z str_l )) ,
+  ((( &( "n" ) )) # Int  |->_)
+  **  ((( &( "paren_string" ) )) # Ptr  |-> paren_string_pre)
+  **  (store_string paren_string_pre str_l )
+|--
+  “ (valid_string str_l ) ” 
+  &&  “ ((string_length (str_l)) < INT_MAX) ”
+.
+
+Definition parse_nested_parens_partial_solve_wit_1_aux := 
+forall (paren_string_pre: Z) (str_l: (@list Z)) (PreH1 : (valid_string str_l )) (PreH2 : (all_ascii str_l )) (PreH3 : (valid_paren_depth_input_6 str_l )) (PreH4 : (parse_safe_input_6 str_l )) (PreH5 : (((string_length (str_l)) + 1 ) < INT_MAX)) (PreH6 : (problem_6_pre_z str_l )) ,
+  (store_string paren_string_pre str_l )
+|--
+  “ (valid_string str_l ) ” 
+  &&  “ ((string_length (str_l)) < INT_MAX) ” 
+  &&  “ (0 <= ((string_length (str_l)) + 1 )) ” 
+  &&  “ (valid_string str_l ) ” 
+  &&  “ (all_ascii str_l ) ” 
+  &&  “ (valid_paren_depth_input_6 str_l ) ” 
+  &&  “ (parse_safe_input_6 str_l ) ” 
+  &&  “ (((string_length (str_l)) + 1 ) < INT_MAX) ” 
+  &&  “ (problem_6_pre_z str_l ) ”
+  &&  (store_string paren_string_pre str_l )
+.
+
+Definition parse_nested_parens_partial_solve_wit_1 := parse_nested_parens_partial_solve_wit_1_pure -> parse_nested_parens_partial_solve_wit_1_aux.
+
+Definition parse_nested_parens_partial_solve_wit_2 := 
+forall (paren_string_pre: Z) (str_l: (@list Z)) (retval: Z) (PreH1 : (retval = (string_length (str_l)))) (PreH2 : (0 <= ((string_length (str_l)) + 1 ))) (PreH3 : (valid_string str_l )) (PreH4 : (all_ascii str_l )) (PreH5 : (valid_paren_depth_input_6 str_l )) (PreH6 : (parse_safe_input_6 str_l )) (PreH7 : (((string_length (str_l)) + 1 ) < INT_MAX)) (PreH8 : (problem_6_pre_z str_l )) ,
+  (store_string paren_string_pre str_l )
+|--
+  “ (retval = (string_length (str_l))) ” 
+  &&  “ (0 <= ((string_length (str_l)) + 1 )) ” 
+  &&  “ (valid_string str_l ) ” 
+  &&  “ (all_ascii str_l ) ” 
+  &&  “ (valid_paren_depth_input_6 str_l ) ” 
+  &&  “ (parse_safe_input_6 str_l ) ” 
+  &&  “ (((string_length (str_l)) + 1 ) < INT_MAX) ” 
+  &&  “ (problem_6_pre_z str_l ) ”
+  &&  (CharArray.full paren_string_pre ((string_length (str_l)) + 1 ) (c_string (str_l)) )
+.
+
+Definition parse_nested_parens_partial_solve_wit_3_pure := 
+(
+forall (paren_string_pre: Z) (str_l: (@list Z)) (retval: Z) (retval_2: Z) (PreH1 : (retval_2 <> 0)) (PreH2 : (retval = (string_length (str_l)))) (PreH3 : (0 <= ((string_length (str_l)) + 1 ))) (PreH4 : (valid_string str_l )) (PreH5 : (all_ascii str_l )) (PreH6 : (valid_paren_depth_input_6 str_l )) (PreH7 : (parse_safe_input_6 str_l )) (PreH8 : (((string_length (str_l)) + 1 ) < INT_MAX)) (PreH9 : (problem_6_pre_z str_l )) ,
+  ((( &( "data" ) )) # Ptr  |->_)
+  **  ((( &( "cap" ) )) # Int  |-> (retval + 1 ))
+  **  ((&((retval_2)  # "<anonymous struct>" ->ₛ "data")) # Ptr  |->_)
+  **  ((&((retval_2)  # "<anonymous struct>" ->ₛ "size")) # Int  |->_)
+  **  (CharArray.full paren_string_pre ((string_length (str_l)) + 1 ) (c_string (str_l)) )
+  **  ((( &( "out" ) )) # Ptr  |-> retval_2)
+  **  ((( &( "n" ) )) # Int  |-> retval)
+  **  ((( &( "paren_string" ) )) # Ptr  |-> paren_string_pre)
+|--
+  “ ((retval + 1 ) < INT_MAX) ” 
+  &&  “ ((retval + 1 ) > 0) ”
+) \/
+(
+forall (paren_string_pre: Z) (str_l: (@list Z)) (retval: Z) (retval_2: Z) (PreH1 : (retval <= INT_MAX)) (PreH2 : ((retval + 1 ) <= INT_MAX)) (PreH3 : (retval >= INT_MIN)) (PreH4 : ((retval + 1 ) >= INT_MIN)) (PreH5 : (retval_2 <> 0)) (PreH6 : (retval = (string_length (str_l)))) (PreH7 : (0 <= ((string_length (str_l)) + 1 ))) (PreH8 : (valid_string str_l )) (PreH9 : (all_ascii str_l )) (PreH10 : (valid_paren_depth_input_6 str_l )) (PreH11 : (parse_safe_input_6 str_l )) (PreH12 : (((string_length (str_l)) + 1 ) < INT_MAX)) (PreH13 : (problem_6_pre_z str_l )) ,
+  ((( &( "data" ) )) # Ptr  |->_)
+  **  ((( &( "cap" ) )) # Int  |-> (retval + 1 ))
+  **  ((&((retval_2)  # "<anonymous struct>" ->ₛ "data")) # Ptr  |->_)
+  **  ((&((retval_2)  # "<anonymous struct>" ->ₛ "size")) # Int  |->_)
+  **  (CharArray.full paren_string_pre ((string_length (str_l)) + 1 ) (c_string (str_l)) )
+  **  ((( &( "out" ) )) # Ptr  |-> retval_2)
+  **  ((( &( "n" ) )) # Int  |-> retval)
+  **  ((( &( "paren_string" ) )) # Ptr  |-> paren_string_pre)
+|--
+  “ ((retval + 1 ) > 0) ”
+).
+
+Definition parse_nested_parens_partial_solve_wit_3_pure_split_goal_1 := 
+forall (paren_string_pre: Z) (str_l: (@list Z)) (retval: Z) (retval_2: Z) (PreH1 : (retval <= INT_MAX)) (PreH2 : ((retval + 1 ) <= INT_MAX)) (PreH3 : (retval >= INT_MIN)) (PreH4 : ((retval + 1 ) >= INT_MIN)) (PreH5 : (retval_2 <> 0)) (PreH6 : (retval = (string_length (str_l)))) (PreH7 : (0 <= ((string_length (str_l)) + 1 ))) (PreH8 : (valid_string str_l )) (PreH9 : (all_ascii str_l )) (PreH10 : (valid_paren_depth_input_6 str_l )) (PreH11 : (parse_safe_input_6 str_l )) (PreH12 : (((string_length (str_l)) + 1 ) < INT_MAX)) (PreH13 : (problem_6_pre_z str_l )) ,
+  ((( &( "data" ) )) # Ptr  |->_)
+  **  ((( &( "cap" ) )) # Int  |-> (retval + 1 ))
+  **  ((&((retval_2)  # "<anonymous struct>" ->ₛ "data")) # Ptr  |->_)
+  **  ((&((retval_2)  # "<anonymous struct>" ->ₛ "size")) # Int  |->_)
+  **  (CharArray.full paren_string_pre ((string_length (str_l)) + 1 ) (c_string (str_l)) )
+  **  ((( &( "out" ) )) # Ptr  |-> retval_2)
+  **  ((( &( "n" ) )) # Int  |-> retval)
+  **  ((( &( "paren_string" ) )) # Ptr  |-> paren_string_pre)
+|--
+  “ ((retval + 1 ) > 0) ”
+.
+
+Definition parse_nested_parens_partial_solve_wit_3_aux := 
+forall (paren_string_pre: Z) (str_l: (@list Z)) (retval: Z) (retval_2: Z) (PreH1 : (retval_2 <> 0)) (PreH2 : (retval = (string_length (str_l)))) (PreH3 : (0 <= ((string_length (str_l)) + 1 ))) (PreH4 : (valid_string str_l )) (PreH5 : (all_ascii str_l )) (PreH6 : (valid_paren_depth_input_6 str_l )) (PreH7 : (parse_safe_input_6 str_l )) (PreH8 : (((string_length (str_l)) + 1 ) < INT_MAX)) (PreH9 : (problem_6_pre_z str_l )) ,
+  ((&((retval_2)  # "<anonymous struct>" ->ₛ "data")) # Ptr  |->_)
+  **  ((&((retval_2)  # "<anonymous struct>" ->ₛ "size")) # Int  |->_)
+  **  (CharArray.full paren_string_pre ((string_length (str_l)) + 1 ) (c_string (str_l)) )
+|--
+  “ ((retval + 1 ) < INT_MAX) ” 
+  &&  “ ((retval + 1 ) > 0) ” 
+  &&  “ (retval_2 <> 0) ” 
+  &&  “ (retval = (string_length (str_l))) ” 
+  &&  “ (0 <= ((string_length (str_l)) + 1 )) ” 
+  &&  “ (valid_string str_l ) ” 
+  &&  “ (all_ascii str_l ) ” 
+  &&  “ (valid_paren_depth_input_6 str_l ) ” 
+  &&  “ (parse_safe_input_6 str_l ) ” 
+  &&  “ (((string_length (str_l)) + 1 ) < INT_MAX) ” 
+  &&  “ (problem_6_pre_z str_l ) ”
+  &&  ((&((retval_2)  # "<anonymous struct>" ->ₛ "data")) # Ptr  |->_)
+  **  ((&((retval_2)  # "<anonymous struct>" ->ₛ "size")) # Int  |->_)
+  **  (CharArray.full paren_string_pre ((string_length (str_l)) + 1 ) (c_string (str_l)) )
+.
+
+Definition parse_nested_parens_partial_solve_wit_3 := parse_nested_parens_partial_solve_wit_3_pure -> parse_nested_parens_partial_solve_wit_3_aux.
+
+Definition parse_nested_parens_partial_solve_wit_4 := 
+forall (paren_string_pre: Z) (str_l: (@list Z)) (ch: Z) (max_level: Z) (level: Z) (output_l: (@list Z)) (out_size: Z) (data: Z) (out: Z) (cap: Z) (n: Z) (i: Z) (PreH1 : ((level - 1 ) = 0)) (PreH2 : ((Znth i (c_string (str_l)) 0) = 41)) (PreH3 : ((Znth i (c_string (str_l)) 0) <> 40)) (PreH4 : (i < n)) (PreH5 : (0 <= i)) (PreH6 : (i <= n)) (PreH7 : (n = (string_length (str_l)))) (PreH8 : (cap = (n + 1 ))) (PreH9 : (out <> 0)) (PreH10 : (data <> 0)) (PreH11 : (0 <= out_size)) (PreH12 : (out_size <= i)) (PreH13 : (out_size = (Zlength (output_l)))) (PreH14 : (0 <= level)) (PreH15 : (level <= i)) (PreH16 : (0 <= max_level)) (PreH17 : (max_level <= i)) (PreH18 : (0 <= ch)) (PreH19 : (ch <= 127)) (PreH20 : (valid_string str_l )) (PreH21 : (all_ascii str_l )) (PreH22 : (valid_paren_depth_input_6 str_l )) (PreH23 : (parse_safe_input_6 str_l )) (PreH24 : (((string_length (str_l)) + 1 ) < INT_MAX)) (PreH25 : (problem_6_pre_z str_l )) (PreH26 : (parse_state_6 str_l i level max_level output_l )) ,
+  (store_string paren_string_pre str_l )
+  **  ((&((out)  # "<anonymous struct>" ->ₛ "data")) # Ptr  |->_)
+  **  ((&((out)  # "<anonymous struct>" ->ₛ "size")) # Int  |->_)
+  **  (IntArray.seg data 0 out_size output_l )
+  **  (IntArray.undef_seg data out_size cap )
+|--
+  “ (0 <= ((string_length (str_l)) + 1 )) ” 
+  &&  “ ((level - 1 ) = 0) ” 
+  &&  “ ((Znth i (c_string (str_l)) 0) = 41) ” 
+  &&  “ ((Znth i (c_string (str_l)) 0) <> 40) ” 
+  &&  “ (i < n) ” 
+  &&  “ (0 <= i) ” 
+  &&  “ (i <= n) ” 
+  &&  “ (n = (string_length (str_l))) ” 
+  &&  “ (cap = (n + 1 )) ” 
+  &&  “ (out <> 0) ” 
+  &&  “ (data <> 0) ” 
+  &&  “ (0 <= out_size) ” 
+  &&  “ (out_size <= i) ” 
+  &&  “ (out_size = (Zlength (output_l))) ” 
+  &&  “ (0 <= level) ” 
+  &&  “ (level <= i) ” 
+  &&  “ (0 <= max_level) ” 
+  &&  “ (max_level <= i) ” 
+  &&  “ (0 <= ch) ” 
+  &&  “ (ch <= 127) ” 
+  &&  “ (valid_string str_l ) ” 
+  &&  “ (all_ascii str_l ) ” 
+  &&  “ (valid_paren_depth_input_6 str_l ) ” 
+  &&  “ (parse_safe_input_6 str_l ) ” 
+  &&  “ (((string_length (str_l)) + 1 ) < INT_MAX) ” 
+  &&  “ (problem_6_pre_z str_l ) ” 
+  &&  “ (parse_state_6 str_l i level max_level output_l ) ”
+  &&  (((data + (out_size * sizeof(INT) ) )) # Int  |->_)
+  **  (CharArray.full paren_string_pre ((string_length (str_l)) + 1 ) (c_string (str_l)) )
+  **  (IntArray.undef_seg data (out_size + 1 ) cap )
+  **  ((&((out)  # "<anonymous struct>" ->ₛ "data")) # Ptr  |->_)
+  **  ((&((out)  # "<anonymous struct>" ->ₛ "size")) # Int  |->_)
+  **  (IntArray.seg data 0 out_size output_l )
+.
+
+Module Type VC_Correct.
+
+Include int_array_Strategy_Correct.
+Include uint_array_Strategy_Correct.
+Include undef_uint_array_Strategy_Correct.
+Include array_shape_Strategy_Correct.
+Include char_array_Strategy_Correct.
+Include string_Strategy_Correct.
+
+Axiom proof_of_parse_nested_parens_safety_wit_1 : parse_nested_parens_safety_wit_1.
+Axiom proof_of_parse_nested_parens_safety_wit_2 : parse_nested_parens_safety_wit_2.
+Axiom proof_of_parse_nested_parens_safety_wit_3 : parse_nested_parens_safety_wit_3.
+Axiom proof_of_parse_nested_parens_safety_wit_4 : parse_nested_parens_safety_wit_4.
+Axiom proof_of_parse_nested_parens_safety_wit_5 : parse_nested_parens_safety_wit_5.
+Axiom proof_of_parse_nested_parens_safety_wit_6 : parse_nested_parens_safety_wit_6.
+Axiom proof_of_parse_nested_parens_safety_wit_7 : parse_nested_parens_safety_wit_7.
+Axiom proof_of_parse_nested_parens_safety_wit_8 : parse_nested_parens_safety_wit_8.
+Axiom proof_of_parse_nested_parens_safety_wit_9 : parse_nested_parens_safety_wit_9.
+Axiom proof_of_parse_nested_parens_safety_wit_10 : parse_nested_parens_safety_wit_10.
+Axiom proof_of_parse_nested_parens_safety_wit_11 : parse_nested_parens_safety_wit_11.
+Axiom proof_of_parse_nested_parens_safety_wit_12 : parse_nested_parens_safety_wit_12.
+Axiom proof_of_parse_nested_parens_safety_wit_13 : parse_nested_parens_safety_wit_13.
+Axiom proof_of_parse_nested_parens_safety_wit_14 : parse_nested_parens_safety_wit_14.
+Axiom proof_of_parse_nested_parens_safety_wit_15 : parse_nested_parens_safety_wit_15.
+Axiom proof_of_parse_nested_parens_safety_wit_16 : parse_nested_parens_safety_wit_16.
+Axiom proof_of_parse_nested_parens_safety_wit_17 : parse_nested_parens_safety_wit_17.
+Axiom proof_of_parse_nested_parens_safety_wit_18 : parse_nested_parens_safety_wit_18.
+Axiom proof_of_parse_nested_parens_safety_wit_19 : parse_nested_parens_safety_wit_19.
+Axiom proof_of_parse_nested_parens_safety_wit_20 : parse_nested_parens_safety_wit_20.
+Axiom proof_of_parse_nested_parens_safety_wit_21 : parse_nested_parens_safety_wit_21.
+Axiom proof_of_parse_nested_parens_entail_wit_1 : parse_nested_parens_entail_wit_1.
+Axiom proof_of_parse_nested_parens_entail_wit_2_1 : parse_nested_parens_entail_wit_2_1.
+Axiom proof_of_parse_nested_parens_entail_wit_2_2 : parse_nested_parens_entail_wit_2_2.
+Axiom proof_of_parse_nested_parens_entail_wit_3 : parse_nested_parens_entail_wit_3.
+Axiom proof_of_parse_nested_parens_entail_wit_4 : parse_nested_parens_entail_wit_4.
+Axiom proof_of_parse_nested_parens_entail_wit_5 : parse_nested_parens_entail_wit_5.
+Axiom proof_of_parse_nested_parens_entail_wit_6_1 : parse_nested_parens_entail_wit_6_1.
+Axiom proof_of_parse_nested_parens_entail_wit_6_2 : parse_nested_parens_entail_wit_6_2.
+Axiom proof_of_parse_nested_parens_entail_wit_6_3 : parse_nested_parens_entail_wit_6_3.
+Axiom proof_of_parse_nested_parens_entail_wit_6_4 : parse_nested_parens_entail_wit_6_4.
+Axiom proof_of_parse_nested_parens_entail_wit_7 : parse_nested_parens_entail_wit_7.
+Axiom proof_of_parse_nested_parens_entail_wit_8 : parse_nested_parens_entail_wit_8.
+Axiom proof_of_parse_nested_parens_return_wit_1 : parse_nested_parens_return_wit_1.
+Axiom proof_of_parse_nested_parens_partial_solve_wit_1_pure : parse_nested_parens_partial_solve_wit_1_pure.
+Axiom proof_of_parse_nested_parens_partial_solve_wit_1 : parse_nested_parens_partial_solve_wit_1.
+Axiom proof_of_parse_nested_parens_partial_solve_wit_2 : parse_nested_parens_partial_solve_wit_2.
+Axiom proof_of_parse_nested_parens_partial_solve_wit_3_pure : parse_nested_parens_partial_solve_wit_3_pure.
+Axiom proof_of_parse_nested_parens_partial_solve_wit_3 : parse_nested_parens_partial_solve_wit_3.
+Axiom proof_of_parse_nested_parens_partial_solve_wit_4 : parse_nested_parens_partial_solve_wit_4.
+
+End VC_Correct.
