QCP_examples/humaneval/spec_logic_rewrite_c_files/C_6_proof_auto.v
@@ -1,0 +1,116 @@
+Require Import Coq.ZArith.ZArith.
+Require Import Coq.Bool.Bool.
+Require Import Coq.Strings.String.
+Require Import Coq.Strings.Ascii.
+Require Import Coq.Lists.List.
+Require Import Coq.Classes.RelationClasses.
+Require Import Coq.Classes.Morphisms.
+Require Import Coq.micromega.Psatz.
+Require Import Coq.Sorting.Permutation.
+From AUXLib Require Import int_auto Axioms Feq Idents ListLib VMap.
+Require Import SetsClass.SetsClass. Import SetsNotation.
+From SimpleC.SL Require Import Mem SeparationLogic.
+From SimpleC.EE Require Import C_6_goal.
+Require Import Logic.LogicGenerator.demo932.Interface.
+Local Open Scope Z_scope.
+Local Open Scope sets.
+Local Open Scope string_scope.
+Local Open Scope list.
+Import naive_C_Rules.
+Require Import SimpleC.StdLib.string_lib.
+Require Import coins_6.
+Local Open Scope sac.
+
+Lemma proof_of_parse_nested_parens_safety_wit_1 : parse_nested_parens_safety_wit_1.
+Proof. Admitted. 
+
+Lemma proof_of_parse_nested_parens_safety_wit_2 : parse_nested_parens_safety_wit_2.
+Proof. Admitted. 
+
+Lemma proof_of_parse_nested_parens_safety_wit_3 : parse_nested_parens_safety_wit_3.
+Proof. Admitted. 
+
+Lemma proof_of_parse_nested_parens_safety_wit_4 : parse_nested_parens_safety_wit_4.
+Proof. Admitted. 
+
+Lemma proof_of_parse_nested_parens_safety_wit_5 : parse_nested_parens_safety_wit_5.
+Proof. Admitted. 
+
+Lemma proof_of_parse_nested_parens_safety_wit_6 : parse_nested_parens_safety_wit_6.
+Proof. Admitted. 
+
+Lemma proof_of_parse_nested_parens_safety_wit_7 : parse_nested_parens_safety_wit_7.
+Proof. Admitted. 
+
+Lemma proof_of_parse_nested_parens_safety_wit_8 : parse_nested_parens_safety_wit_8.
+Proof. Admitted. 
+
+Lemma proof_of_parse_nested_parens_safety_wit_9 : parse_nested_parens_safety_wit_9.
+Proof. Admitted. 
+
+Lemma proof_of_parse_nested_parens_safety_wit_10 : parse_nested_parens_safety_wit_10.
+Proof. Admitted. 
+
+Lemma proof_of_parse_nested_parens_safety_wit_11 : parse_nested_parens_safety_wit_11.
+Proof. Admitted. 
+
+Lemma proof_of_parse_nested_parens_safety_wit_12 : parse_nested_parens_safety_wit_12.
+Proof. Admitted. 
+
+Lemma proof_of_parse_nested_parens_safety_wit_13 : parse_nested_parens_safety_wit_13.
+Proof. Admitted. 
+
+Lemma proof_of_parse_nested_parens_safety_wit_14 : parse_nested_parens_safety_wit_14.
+Proof. Admitted. 
+
+Lemma proof_of_parse_nested_parens_safety_wit_15 : parse_nested_parens_safety_wit_15.
+Proof. Admitted. 
+
+Lemma proof_of_parse_nested_parens_safety_wit_16 : parse_nested_parens_safety_wit_16.
+Proof. Admitted. 
+
+Lemma proof_of_parse_nested_parens_safety_wit_17 : parse_nested_parens_safety_wit_17.
+Proof. Admitted. 
+
+Lemma proof_of_parse_nested_parens_safety_wit_18 : parse_nested_parens_safety_wit_18.
+Proof. Admitted. 
+
+Lemma proof_of_parse_nested_parens_safety_wit_19 : parse_nested_parens_safety_wit_19.
+Proof. Admitted. 
+
+Lemma proof_of_parse_nested_parens_safety_wit_20 : parse_nested_parens_safety_wit_20.
+Proof. Admitted. 
+
+Lemma proof_of_parse_nested_parens_safety_wit_21 : parse_nested_parens_safety_wit_21.
+Proof. Admitted. 
+
+Lemma proof_of_parse_nested_parens_entail_wit_6_1 : parse_nested_parens_entail_wit_6_1.
+Proof. Admitted. 
+
+Lemma proof_of_parse_nested_parens_entail_wit_6_2 : parse_nested_parens_entail_wit_6_2.
+Proof. Admitted. 
+
+Lemma proof_of_parse_nested_parens_entail_wit_6_3 : parse_nested_parens_entail_wit_6_3.
+Proof. Admitted. 
+
+Lemma proof_of_parse_nested_parens_entail_wit_6_4 : parse_nested_parens_entail_wit_6_4.
+Proof. Admitted. 
+
+Lemma proof_of_parse_nested_parens_entail_wit_8 : parse_nested_parens_entail_wit_8.
+Proof. Admitted. 
+
+Lemma proof_of_parse_nested_parens_partial_solve_wit_1_pure : parse_nested_parens_partial_solve_wit_1_pure.
+Proof. Admitted. 
+
+Lemma proof_of_parse_nested_parens_partial_solve_wit_1 : parse_nested_parens_partial_solve_wit_1.
+Proof. Admitted. 
+
+Lemma proof_of_parse_nested_parens_partial_solve_wit_2 : parse_nested_parens_partial_solve_wit_2.
+Proof. Admitted. 
+
+Lemma proof_of_parse_nested_parens_partial_solve_wit_3 : parse_nested_parens_partial_solve_wit_3.
+Proof. Admitted. 
+
+Lemma proof_of_parse_nested_parens_partial_solve_wit_4 : parse_nested_parens_partial_solve_wit_4.
+Proof. Admitted. 
+
