QCP_examples/humaneval/spec_logic_rewrite_c_files/C_6_proof_manual.v
@@ -1,0 +1,140 @@
+Require Import Coq.ZArith.ZArith.
+Require Import Coq.Bool.Bool.
+Require Import Coq.Strings.String.
+Require Import Coq.Strings.Ascii.
+Require Import Coq.Lists.List.
+Require Import Coq.Classes.RelationClasses.
+Require Import Coq.Classes.Morphisms.
+Require Import Coq.micromega.Psatz.
+Require Import Coq.Sorting.Permutation.
+From AUXLib Require Import int_auto Axioms Feq Idents ListLib VMap.
+Require Import SetsClass.SetsClass. Import SetsNotation.
+From SimpleC.SL Require Import Mem SeparationLogic.
+From SimpleC.EE Require Import C_6_goal.
+From SimpleC.EE Require Import C_6_proof_auto.
+Require Import Logic.LogicGenerator.demo932.Interface.
+Local Open Scope Z_scope.
+Local Open Scope sets.
+Local Open Scope string_scope.
+Local Open Scope list.
+Import naive_C_Rules.
+Require Import SimpleC.StdLib.string_lib.
+Require Import coins_6.
+Local Open Scope sac.
+
+Ltac solve_len_6 :=
+  unfold SimpleC.StdLib.string_lib.string_length, coins_6.string_length in *; lia.
+
+Lemma proof_of_parse_nested_parens_entail_wit_1 : parse_nested_parens_entail_wit_1.
+Proof.
+  right; intros.
+  pre_process.
+  entailer!;
+    try apply parse_state_6_initial;
+    try (subst retval; unfold SimpleC.StdLib.string_lib.string_length, coins_6.string_length; apply Zlength_nonneg);
+    try solve_len_6.
+Qed.
+
+Lemma proof_of_parse_nested_parens_entail_wit_2_1 : parse_nested_parens_entail_wit_2_1.
+Proof.
+  right; intros.
+  pre_process.
+  entailer!.
+  rewrite c_string_Znth_inside in PreH3 by solve_len_6.
+  pose proof (parse_state_6_step_open
+                str_l i level max_level output_l_2
+                PreH26 PreH3 ltac:(solve_len_6)) as Hstep.
+  replace (Z.max max_level (level + 1)) with max_level in Hstep by lia.
+  exact Hstep.
+Qed.
+
+Lemma proof_of_parse_nested_parens_entail_wit_2_2 : parse_nested_parens_entail_wit_2_2.
+Proof.
+  right; intros.
+  pre_process.
+  entailer!.
+  rewrite c_string_Znth_inside in PreH3 by solve_len_6.
+  pose proof (parse_state_6_step_open
+                str_l i level max_level output_l_2
+                PreH26 PreH3 ltac:(solve_len_6)) as Hstep.
+  replace (Z.max max_level (level + 1)) with (level + 1) in Hstep by lia.
+  exact Hstep.
+Qed.
+
+Lemma proof_of_parse_nested_parens_entail_wit_3 : parse_nested_parens_entail_wit_3.
+Proof.
+  right; intros.
+  pre_process.
+  rewrite c_string_Znth_inside in PreH3 by solve_len_6.
+  assert (Hlevel_one : level = 1) by lia.
+  subst level.
+  entailer!.
+  - rewrite Zlength_app, Zlength_cons, Zlength_nil.
+    lia.
+  - replace (1 - 1) with 0 by lia.
+    eapply parse_state_6_step_close_finish; eauto; solve_len_6.
+Qed.
+
+Lemma proof_of_parse_nested_parens_entail_wit_4 : parse_nested_parens_entail_wit_4.
+Proof.
+  right; intros.
+  pre_process.
+  rewrite c_string_Znth_inside in PreH3 by solve_len_6.
+  assert (Hlevel_pos : 0 < level).
+  {
+    destruct PreH24 as [Hsafe _].
+    assert (0 <= i < Zlength str_l) by solve_len_6.
+    specialize (Hsafe i H PreH3).
+    unfold parse_state_6 in PreH27.
+    destruct PreH27 as [_ [_ [Hlev _]]].
+    lia.
+  }
+  entailer!.
+  eapply parse_state_6_step_close_continue; eauto; solve_len_6.
+Qed.
+
+Lemma proof_of_parse_nested_parens_entail_wit_5 : parse_nested_parens_entail_wit_5.
+Proof.
+  right; intros.
+  pre_process.
+  rewrite c_string_Znth_inside in PreH2 by solve_len_6.
+  rewrite c_string_Znth_inside in PreH3 by solve_len_6.
+  assert (Hspace : Znth i str_l 0 = 32).
+  {
+    destruct (PreH22 i ltac:(solve_len_6)) as [|[|]]; lia.
+  }
+  entailer!.
+  - rewrite c_string_Znth_inside by solve_len_6.
+    exact Hspace.
+  - eapply parse_state_6_step_space; eauto; solve_len_6.
+Qed.
+
+Lemma proof_of_parse_nested_parens_entail_wit_7 : parse_nested_parens_entail_wit_7.
+Proof.
+  right; intros.
+  pre_process.
+  assert (Hend : i >= string_length str_l) by lia.
+  destruct (parse_state_6_final_facts
+              str_l i level max_level output_l_2 PreH24 PreH21 Hend)
+    as [Hlevel [Hmax [Hout Hspec]]].
+  subst.
+  entailer!.
+Qed.
+
+Lemma proof_of_parse_nested_parens_return_wit_1 : parse_nested_parens_return_wit_1.
+Proof.
+  right; intros.
+  pre_process.
+  subst.
+  entailer!.
+Qed.
+
+Lemma proof_of_parse_nested_parens_partial_solve_wit_3_pure : parse_nested_parens_partial_solve_wit_3_pure.
+Proof.
+  right; intros.
+  pre_process; entailer!.
+  subst retval.
+  unfold SimpleC.StdLib.string_lib.string_length, coins_6.string_length in *.
+  pose proof (Zlength_nonneg str_l).
+  lia.
+Qed.
