QCP_examples/humaneval/spec_logic_rewrite_c_files/coins_6.v
@@ -1,0 +1,329 @@
+Load "../spec/6".
+
+Require Import Coq.ZArith.ZArith.
+Require Import Coq.Lists.List.
+Require Import Coq.Strings.String.
+Require Import Coq.Strings.Ascii.
+Require Import Lia.
+From AUXLib Require Import ListLib.
+From SimpleC.SL Require Import IntLib.
+
+Import ListNotations.
+
+Local Open Scope Z_scope.
+Local Open Scope string_scope.
+Local Open Scope list_scope.
+
+Definition ascii_of_z_6 (z : Z) : ascii :=
+  ascii_of_nat (Z.to_nat z).
+
+Fixpoint string_of_list_z (l : list Z) : string :=
+  match l with
+  | [] => EmptyString
+  | c :: rest => String (ascii_of_z_6 c) (string_of_list_z rest)
+  end.
+
+Definition string_length (s : list Z) : Z :=
+  Zlength s.
+
+Definition problem_6_pre_z (s : list Z) : Prop :=
+  problem_6_pre (string_of_list_z s).
+
+Definition problem_6_spec_z (s output : list Z) : Prop :=
+  problem_6_spec (string_of_list_z s) (map Z.to_nat output).
+
+Definition valid_paren_depth_char_6 (c : Z) : Prop :=
+  c = 32 \/ c = 40 \/ c = 41.
+
+Definition valid_paren_depth_input_6 (s : list Z) : Prop :=
+  forall i, 0 <= i < Zlength s -> valid_paren_depth_char_6 (Znth i s 0).
+
+Definition depth_step_6
+    (st : list Z * Z * Z) (c : Z) : list Z * Z * Z :=
+  let '(levels, level, max_level) := st in
+  if Z.eqb c 40 then
+    let level' := level + 1 in
+    (levels, level', Z.max max_level level')
+  else if Z.eqb c 41 then
+    let level' := level - 1 in
+    if Z.eqb level' 0 then
+      (levels ++ [max_level], 0, 0)
+    else (levels, level', max_level)
+  else (levels, level, max_level).
+
+Fixpoint depth_state_nat_6 (n : nat) (s : list Z) : list Z * Z * Z :=
+  match n with
+  | O => ([], 0, 0)
+  | S n' =>
+      depth_step_6
+        (depth_state_nat_6 n' s)
+        (Znth (Z.of_nat n') s 0)
+  end.
+
+Definition depth_completed_6 (s : list Z) (i : Z) : list Z :=
+  let '(levels, _, _) := depth_state_nat_6 (Z.to_nat i) s in levels.
+
+Definition depth_level_6 (s : list Z) (i : Z) : Z :=
+  let '(_, level, _) := depth_state_nat_6 (Z.to_nat i) s in level.
+
+Definition depth_max_6 (s : list Z) (i : Z) : Z :=
+  let '(_, _, max_level) := depth_state_nat_6 (Z.to_nat i) s in max_level.
+
+Definition parse_output_6 (s : list Z) : list Z :=
+  depth_completed_6 s (Zlength s).
+
+Definition parse_state_6
+    (s : list Z) (i level max_level : Z) (output : list Z) : Prop :=
+  0 <= i <= string_length s /\
+  output = depth_completed_6 s i /\
+  level = depth_level_6 s i /\
+  max_level = depth_max_6 s i /\
+  0 <= level /\
+  0 <= max_level /\
+  Zlength output <= i.
+
+Definition parse_safe_input_6 (s : list Z) : Prop :=
+  (forall i,
+    0 <= i < Zlength s ->
+    Znth i s 0 = 41 ->
+    0 < depth_level_6 s i) /\
+  depth_level_6 s (Zlength s) = 0 /\
+  depth_max_6 s (Zlength s) = 0 /\
+  problem_6_spec_z s (parse_output_6 s).
+
+Lemma depth_state_nat_6_step : forall i s,
+  0 <= i ->
+  depth_state_nat_6 (Z.to_nat (i + 1)) s =
+  depth_step_6 (depth_state_nat_6 (Z.to_nat i) s) (Znth i s 0).
+Proof.
+  intros i s Hi.
+  replace (Z.to_nat (i + 1)) with (S (Z.to_nat i)) by lia.
+  simpl.
+  replace (Z.of_nat (Z.to_nat i)) with i by lia.
+  reflexivity.
+Qed.
+
+Lemma parse_state_6_initial : forall s,
+  parse_state_6 s 0 0 0 [].
+Proof.
+  intros s.
+  unfold parse_state_6, depth_completed_6, depth_level_6, depth_max_6, string_length.
+  simpl.
+  repeat split; try reflexivity; try rewrite Zlength_nil; try lia; apply Zlength_nonneg.
+Qed.
+
+Lemma parse_state_6_step_open : forall s i level max_level output,
+  parse_state_6 s i level max_level output ->
+  Znth i s 0 = 40 ->
+  i < Zlength s ->
+  parse_state_6 s (i + 1) (level + 1) (Z.max max_level (level + 1)) output.
+Proof.
+  intros s i level max_level output Hstate Hch Hi.
+  unfold parse_state_6 in *.
+  destruct Hstate as [Hbounds [Hout [Hlev [Hmax [Hlevnon [Hmaxnon Hlen]]]]]].
+  repeat split; try (unfold string_length in *; lia).
+  - unfold depth_completed_6 in *.
+    rewrite depth_state_nat_6_step by lia.
+    destruct (depth_state_nat_6 (Z.to_nat i) s) as [[levels0 level0] max0] eqn:Hst.
+    unfold depth_level_6 in Hlev; rewrite Hst in Hlev.
+    unfold depth_max_6 in Hmax; rewrite Hst in Hmax.
+    subst output level max_level.
+    simpl in *.
+    unfold depth_step_6.
+    rewrite Hch, Z.eqb_refl.
+    reflexivity.
+  - unfold depth_level_6.
+    rewrite depth_state_nat_6_step by lia.
+    destruct (depth_state_nat_6 (Z.to_nat i) s) as [[levels0 level0] max0] eqn:Hst.
+    unfold depth_level_6 in Hlev; rewrite Hst in Hlev.
+    subst level.
+    simpl in *.
+    unfold depth_step_6.
+    rewrite Hch, Z.eqb_refl.
+    reflexivity.
+  - unfold depth_max_6.
+    rewrite depth_state_nat_6_step by lia.
+    destruct (depth_state_nat_6 (Z.to_nat i) s) as [[levels0 level0] max0] eqn:Hst.
+    unfold depth_level_6 in Hlev; rewrite Hst in Hlev.
+    unfold depth_max_6 in Hmax; rewrite Hst in Hmax.
+    subst level max_level.
+    simpl in *.
+    unfold depth_step_6.
+    rewrite Hch, Z.eqb_refl.
+    reflexivity.
+Qed.
+
+Lemma parse_state_6_step_close_finish : forall s i max_level output,
+  parse_state_6 s i 1 max_level output ->
+  Znth i s 0 = 41 ->
+  i < Zlength s ->
+  parse_state_6 s (i + 1) 0 0 (output ++ [max_level]).
+Proof.
+  intros s i max_level output Hstate Hch Hi.
+  unfold parse_state_6 in *.
+  destruct Hstate as [Hbounds [Hout [Hlev [Hmax [Hlevnon [Hmaxnon Hlen]]]]]].
+  repeat split; try (unfold string_length in *; lia).
+  - unfold depth_completed_6 in *.
+    rewrite depth_state_nat_6_step by lia.
+    destruct (depth_state_nat_6 (Z.to_nat i) s) as [[levels0 level0] max0] eqn:Hst.
+    simpl in *.
+    unfold depth_level_6 in Hlev; rewrite Hst in Hlev.
+    unfold depth_max_6 in Hmax; rewrite Hst in Hmax.
+    subst output max_level.
+    unfold depth_step_6.
+    rewrite Hch.
+    replace (Z.eqb 41 40) with false by reflexivity.
+    replace (level0 - 1) with 0 by lia.
+    rewrite Z.eqb_refl.
+    reflexivity.
+  - unfold depth_level_6.
+    rewrite depth_state_nat_6_step by lia.
+    destruct (depth_state_nat_6 (Z.to_nat i) s) as [[levels0 level0] max0] eqn:Hst.
+    simpl in *.
+    unfold depth_step_6.
+    rewrite Hch.
+    replace (Z.eqb 41 40) with false by reflexivity.
+    unfold depth_level_6 in Hlev; rewrite Hst in Hlev.
+    replace (level0 - 1) with 0 by lia.
+    rewrite Z.eqb_refl.
+    reflexivity.
+  - unfold depth_max_6.
+    rewrite depth_state_nat_6_step by lia.
+    destruct (depth_state_nat_6 (Z.to_nat i) s) as [[levels0 level0] max0] eqn:Hst.
+    simpl in *.
+    unfold depth_step_6.
+    rewrite Hch.
+    replace (Z.eqb 41 40) with false by reflexivity.
+    unfold depth_level_6 in Hlev; rewrite Hst in Hlev.
+    replace (level0 - 1) with 0 by lia.
+    rewrite Z.eqb_refl.
+    reflexivity.
+  - rewrite Zlength_app, Zlength_cons, Zlength_nil.
+    lia.
+Qed.
+
+Lemma parse_state_6_step_close_continue : forall s i level max_level output,
+  parse_state_6 s i level max_level output ->
+  parse_safe_input_6 s ->
+  level - 1 <> 0 ->
+  Znth i s 0 = 41 ->
+  i < Zlength s ->
+  parse_state_6 s (i + 1) (level - 1) max_level output.
+Proof.
+  intros s i level max_level output Hstate Hsafe Hnot0 Hch Hi.
+  unfold parse_state_6 in *.
+  destruct Hstate as [Hbounds [Hout [Hlev [Hmax [Hlevnon [Hmaxnon Hlen]]]]]].
+  assert (Hpos : 0 < level).
+  {
+    destruct Hsafe as [Hsafe _].
+    assert (0 <= i < Zlength s) as Hi_bounds by (unfold string_length in *; lia).
+    specialize (Hsafe i Hi_bounds Hch).
+    lia.
+  }
+  repeat split; try (unfold string_length in *; lia).
+  - unfold depth_completed_6 in *.
+    rewrite depth_state_nat_6_step by lia.
+    destruct (depth_state_nat_6 (Z.to_nat i) s) as [[levels0 level0] max0] eqn:Hst.
+    simpl in *.
+    unfold depth_level_6 in Hlev; rewrite Hst in Hlev.
+    unfold depth_max_6 in Hmax; rewrite Hst in Hmax.
+    subst output level max_level.
+    unfold depth_step_6.
+    rewrite Hch.
+    replace (Z.eqb 41 40) with false by reflexivity.
+    destruct (Z.eqb_spec (level0 - 1) 0); [lia | reflexivity].
+  - unfold depth_level_6.
+    rewrite depth_state_nat_6_step by lia.
+    destruct (depth_state_nat_6 (Z.to_nat i) s) as [[levels0 level0] max0] eqn:Hst.
+    unfold depth_level_6 in Hlev; rewrite Hst in Hlev.
+    subst level.
+    simpl in *.
+    unfold depth_step_6.
+    rewrite Hch.
+    replace (Z.eqb 41 40) with false by reflexivity.
+    destruct (Z.eqb_spec (level0 - 1) 0); [lia | reflexivity].
+  - unfold depth_max_6.
+    rewrite depth_state_nat_6_step by lia.
+    destruct (depth_state_nat_6 (Z.to_nat i) s) as [[levels0 level0] max0] eqn:Hst.
+    unfold depth_level_6 in Hlev; rewrite Hst in Hlev.
+    unfold depth_max_6 in Hmax; rewrite Hst in Hmax.
+    subst level max_level.
+    simpl in *.
+    unfold depth_step_6.
+    rewrite Hch.
+    replace (Z.eqb 41 40) with false by reflexivity.
+    destruct (Z.eqb_spec (level0 - 1) 0); [lia |].
+    reflexivity.
+Qed.
+
+Lemma parse_state_6_step_space : forall s i level max_level output,
+  parse_state_6 s i level max_level output ->
+  Znth i s 0 = 32 ->
+  i < Zlength s ->
+  parse_state_6 s (i + 1) level max_level output.
+Proof.
+  intros s i level max_level output Hstate Hch Hi.
+  unfold parse_state_6 in *.
+  destruct Hstate as [Hbounds [Hout [Hlev [Hmax [Hlevnon [Hmaxnon Hlen]]]]]].
+  repeat split; try (unfold string_length in *; lia).
+  - unfold depth_completed_6 in *.
+    rewrite depth_state_nat_6_step by lia.
+    destruct (depth_state_nat_6 (Z.to_nat i) s) as [[levels0 level0] max0] eqn:Hst.
+    simpl in *.
+    subst output level max_level.
+    unfold depth_step_6.
+    rewrite Hch.
+    reflexivity.
+  - unfold depth_level_6.
+    rewrite depth_state_nat_6_step by lia.
+    destruct (depth_state_nat_6 (Z.to_nat i) s) as [[levels0 level0] max0] eqn:Hst.
+    unfold depth_level_6 in Hlev; rewrite Hst in Hlev.
+    subst level.
+    simpl in *.
+    unfold depth_step_6.
+    rewrite Hch.
+    reflexivity.
+  - unfold depth_max_6.
+    rewrite depth_state_nat_6_step by lia.
+    destruct (depth_state_nat_6 (Z.to_nat i) s) as [[levels0 level0] max0] eqn:Hst.
+    unfold depth_max_6 in Hmax; rewrite Hst in Hmax.
+    subst max_level.
+    simpl in *.
+    unfold depth_step_6.
+    rewrite Hch.
+    reflexivity.
+Qed.
+
+Lemma parse_state_6_final_spec : forall s output,
+  parse_state_6 s (Zlength s) 0 0 output ->
+  parse_safe_input_6 s ->
+  problem_6_spec_z s output.
+Proof.
+  intros s output Hstate Hsafe.
+  unfold parse_state_6 in Hstate.
+  destruct Hstate as [_ [Hout _]].
+  destruct Hsafe as [_ [_ [_ Hspec]]].
+  subst output.
+  exact Hspec.
+Qed.
+
+Lemma parse_state_6_final_facts : forall s i level max_level output,
+  parse_state_6 s i level max_level output ->
+  parse_safe_input_6 s ->
+  i >= string_length s ->
+  level = 0 /\
+  max_level = 0 /\
+  output = parse_output_6 s /\
+  problem_6_spec_z s output.
+Proof.
+  intros s i level max_level output Hstate Hsafe Hend.
+  unfold parse_state_6 in Hstate.
+  destruct Hstate as [Hbounds [Hout [Hlev [Hmax _]]]].
+  unfold string_length in *.
+  assert (Hi : i = Zlength s) by lia.
+  subst i.
+  destruct Hsafe as [_ [Hlev_end [Hmax_end Hspec]]].
+  unfold parse_output_6.
+  subst output level max_level.
+  repeat split; auto.
+Qed.
